Modified, and proved termination for nodesValid proved nodesValid_heaps_eq_imp_nodesValid revisited the heap_invs proof, partially updated it

Proofs/Memory.thy
@@ -1,97 +1,111 @@
 theory Memory
-imports
-  "../AutoCorres/Impl"
-  "../lib/ExtraLemmas"
-  "./Memory_Nodes"
-  "~/Isabelle2016-1/src/HOL/Library/LaTeXsugar"
-  
+  imports
+    "../AutoCorres/Impl"
+    "../lib/ExtraLemmas"
+    "./Memory_Nodes"
+    "~/Isabelle2016-1/src/HOL/Library/LaTeXsugar"
+    
 begin
-
+  
 context sable_isa
 begin
-
+  
 abbreviation "ALIGN_BITS \<equiv> 3"
-
+abbreviation "OCC_FLG \<equiv> MEM_NODE_OCCUPIED_FLAG" 
+  
+abbreviation unat_ptr :: "'a ptr \<Rightarrow> nat"
+  where "unat_ptr p \<equiv> unat (ptr_val p)"
+    
 definition
   mem_node_C_guard :: "mem_node_C ptr \<Rightarrow> bool"
-where
-  "mem_node_C_guard n \<equiv> c_null_guard n \<and> is_aligned (ptr_val n) ALIGN_BITS"
-
+  where
+    "mem_node_C_guard n \<equiv> c_null_guard n \<and> is_aligned (ptr_val n) ALIGN_BITS"
+    
 lemma[dest, intro]: "mem_node_C_guard p \<Longrightarrow> c_guard p"
-unfolding mem_node_C_guard_def c_guard_def ptr_aligned_def is_aligned_def
-by (auto simp add: align_of_def, unat_arith)
-
+  unfolding mem_node_C_guard_def c_guard_def ptr_aligned_def is_aligned_def
+  by (auto simp add: align_of_def, unat_arith)
+    
 lemma contrapos: "(P \<longrightarrow> Q) = (\<not>Q \<longrightarrow> \<not>P)"
-by blast
-
+  by blast
+    
 definition
   liftC :: "('c \<Rightarrow> 'a) \<Rightarrow> ('c \<Rightarrow> bool) \<Rightarrow> ('a \<Rightarrow> bool)"
-where
-  "liftC st P \<equiv> \<lambda>s. \<forall>g. s = st g \<longrightarrow> P g"
-
+  where
+    "liftC st P \<equiv> \<lambda>s. \<forall>g. s = st g \<longrightarrow> P g"
+    
 lemma hoare_liftC_wp[wp]:
   "\<lbrace>P\<rbrace> m \<lbrace>\<lambda>r s. \<forall>t. st s = t \<longrightarrow> Q r t\<rbrace> \<Longrightarrow> \<lbrace>liftC st P\<rbrace> exec_concrete st m \<lbrace>Q\<rbrace>"
-unfolding liftC_def
-apply wp
-unfolding valid_def
-apply auto 
-oops
-
+  unfolding liftC_def
+  apply wp
+  unfolding valid_def
+   apply auto 
+  oops
+    
 lemma hoare_liftC[intro]:
   "\<lbrace>P\<rbrace> m \<lbrace>\<lambda>r s. \<forall>t. st s = t \<longrightarrow> liftC st (Q r) t\<rbrace> \<Longrightarrow>
    \<lbrace>liftC st P\<rbrace> exec_concrete st m \<lbrace>\<lambda>r s. liftC st (Q r) s\<rbrace>"
   apply wp
   sorry   
-
+    
 lemma fail'_wp: "\<lbrace>\<lambda>x. True\<rbrace> fail' \<lbrace>Q\<rbrace>"
-unfolding fail'_def FUNCTION_BODY_NOT_IN_INPUT_C_FILE_def by wp
-
-(*definition
+  unfolding fail'_def FUNCTION_BODY_NOT_IN_INPUT_C_FILE_def by wp
+    
+    
+    (*definition
   init_heap_P :: "unit ptr \<Rightarrow> 32 word \<Rightarrow> globals \<Rightarrow> bool"
 where
   "init_heap_P p n s \<equiv> 0 \<notin> {ptr_val p..+unat n} \<and> is_aligned (ptr_val p) ALIGN_BITS \<and>
     (\<forall>node \<in> {ptr_val p..+unat n}. snd (hrs_htd (t_hrs_' s) node) = Map.empty)"*)
     
+    (* FIXME move it out of here *)
+lemma unat_add_le: "unat (a + b) \<le> unat (a::('a::len word)) + unat b "
+  by unat_arith
+    
 definition nodeFree :: "globals \<Rightarrow> mem_node_C ptr \<Rightarrow> bool"
-where "nodeFree s node \<equiv>
-    (let size = (mem_node_C.size_C (h_val (hrs_mem (t_hrs_' s)) node)) && scast (~~ MEM_NODE_OCCUPIED_FLAG) in
+  where "nodeFree s node \<equiv>
+    (let size = node_size_masked s node in
     \<forall>p \<in> {ptr_val (node +\<^sub>p 1)..+unat size * size_of TYPE(mem_node_C)}.
       snd (hrs_htd (t_hrs_' s) p) = Map.empty)"
-
+    
 lemma eight_eq_eight : "unat (8::32 word) = 8" by simp
     
 definition nodeValid :: "globals \<Rightarrow> mem_node_C ptr \<Rightarrow> bool"
-where "nodeValid s node = 
-  (let occupied = node_size s node && scast  MEM_NODE_OCCUPIED_FLAG in
+  where "nodeValid s node = 
+  (let occupied = node_size s node && scast OCC_FLG in
    let next = node_next s node in
    let size = node_size_masked s node in
    c_guard node \<and> 
-   unat (ptr_val node) + 8 + unat (size * 8) \<le> 
-    (if (next \<noteq> NULL) then unat (ptr_val next) else 2 ^ LENGTH(32)) \<and>
+   unat_ptr node + 8 + unat (size * 8) \<le> 
+    (if (next \<noteq> NULL) then unat_ptr next else 2 ^ LENGTH(32)) \<and>
    unat size * 8 < 2 ^ LENGTH(32) \<and>
    (occupied = 0 \<longrightarrow> nodeFree s node) \<and> 
    (next \<noteq> NULL \<longrightarrow> next > node \<and> next \<ge> (node +\<^sub>p 1)) )"
+    
+lemma "c_null_guard p \<Longrightarrow> 
+  x \<in> ptr_span (p::mem_node_C ptr) \<Longrightarrow>
+  unat x < unat_ptr p + size_of (TYPE(mem_node_C))" sorry 
 
 lemma nodeValid_node_size_l1:
-  "nodeValid s node \<Longrightarrow>  unat (ptr_val (node +\<^sub>p 1)) + unat ((node_size_masked s node) * 8) \<le> 
+  "nodeValid s node \<Longrightarrow>  unat_ptr (node +\<^sub>p 1) + unat ((node_size_masked s node) * 8) \<le> 
     2 ^ LENGTH(32)"
   unfolding nodeValid_def Let_def
-      apply (subgoal_tac "unat (ptr_val (next_C (h_val (hrs_mem (t_hrs_' s)) node))) < 2 ^ LENGTH(32)")
+  apply (subgoal_tac "unat (ptr_val (next_C (h_val (hrs_mem (t_hrs_' s)) node))) < 2 ^ LENGTH(32)")
    apply (auto simp:if_split)[1] sorry(* 
   by (metis unat_lt2p word_bits_len_of) *)
-lemma nodeValid_node_size_l1_new:
-  "nodeValid s node \<Longrightarrow>  unat (ptr_val node) + 8 + unat ((node_size_masked s node) * 8) \<le> 
-    2 ^ LENGTH(32)" sorry
     
+lemma nodeValid_node_size_l1_new:
+  "nodeValid s node \<Longrightarrow>  unat_ptr node + 8 + unat ((node_size_masked s node) * 8) \<le> 
+    2 ^ LENGTH(32)" sorry
+  
 lemma nodeValid_node_size_l2:
   "nodeValid s node \<Longrightarrow>  
-   unat (ptr_val (node +\<^sub>p 1)) + unat (node_size_masked s node) * 8 \<le> 2 ^ LENGTH(32)"
+   unat_ptr (node +\<^sub>p 1) + unat (node_size_masked s node) * 8 \<le> 2 ^ LENGTH(32)"
   unfolding nodeValid_def Let_def    
-  apply (subgoal_tac "unat (ptr_val (node_next s node)) < 2 ^ LENGTH(32)")
+  apply (subgoal_tac "unat_ptr (node_next s node) < 2 ^ LENGTH(32)")
    apply (subgoal_tac "unat (node_size_masked s node) * unat (8::word32) =
            unat ((node_size_masked s node) * 8)") 
     apply (auto simp:if_split)[1]
-    sorry(* 
+  sorry(* 
    apply (clarify)
    apply (subst (asm) eight_eq_eight[THEN sym])
    apply (frule unat_mult_lem[THEN iffD1]) 
@@ -99,33 +113,44 @@ lemma nodeValid_node_size_l2:
   using unat_lt2p by blast  *)
 lemma nodeValid_node_size_l2_new:
   "nodeValid s node \<Longrightarrow>  
-   unat (ptr_val node) + 8 + unat (node_size_masked s node) * 8 \<le> 2 ^ LENGTH(32)"
+   unat_ptr node + 8 + unat (node_size_masked s node) * 8 \<le> 2 ^ LENGTH(32)"
   sorry
     
-thm unat_mult_lem[iff]   
+lemma nodeValid_node_size_l3:
+  "nodeValid s node \<Longrightarrow>
+     8 + unat (node_size_masked s node) * 8 < 2 ^ LENGTH(32)"
+  apply (subgoal_tac "ptr_val node > 0")
+   apply (drule nodeValid_node_size_l2_new)
+   apply unat_arith
+  unfolding nodeValid_def Let_def apply clarify
+  apply (drule c_guard_NULL) 
+  apply (subgoal_tac "ptr_val node \<noteq> 0") 
+  using word_neq_0_conv apply blast
+  by (metis ptr.exhaust ptr_val.ptr_val_def)
+    
 function nodesValid :: "globals \<Rightarrow> mem_node_C ptr \<Rightarrow> bool" where
- "\<not> (nodeValid s heap) \<Longrightarrow> nodesValid s heap = False"
+  "\<not> (nodeValid s heap) \<Longrightarrow> nodesValid s heap = False"
 |"nodeValid s heap \<and> node_next s heap = NULL \<Longrightarrow> nodesValid s heap = True"
 |"nodeValid s heap \<and> node_next s heap \<noteq> NULL \<Longrightarrow> nodesValid s heap =
       nodesValid s (node_next s heap)"
-apply auto by blast 
+        apply auto by blast 
 termination
-  apply (relation "measure (\<lambda> (s,heap). 2 ^ 32 - unat (ptr_val heap))")
+  apply (relation "measure (\<lambda> (s,heap). 2 ^ 32 - unat_ptr heap)")
    apply auto
   unfolding nodeValid_def Let_def
   apply (clarsimp simp:ptr_less_simp ptr_le_simp)
   by unat_arith auto
-
-(* FIXME : remove if safe*)    
-(* declare nodesValid.simps[simp del]   *)
-
+    
+    (* FIXME : remove if safe*)    
+    (* declare nodesValid.simps[simp del]   *)
+    
 lemma nodesValid_def' :"nodesValid s heap =
   (let next = (node_next s heap) in 
     nodeValid s heap \<and> (next \<noteq> NULL \<longrightarrow> nodesValid s next))"
   unfolding Let_def
   using nodesValid.simps
   by blast
-
+    
 thm nodesValid.induct    
 lemma nodesValid_induct' :
   "(\<And>s heap.
@@ -134,43 +159,35 @@ lemma nodesValid_induct' :
     P s heap) \<Longrightarrow>
   P s node"    
   sorry
-  
+    
 thm nodesValid.induct
 thm nodesValid.simps
 thm nodesValid_def'
   
 definition heap_invs :: "globals \<Rightarrow> unit ptr \<Rightarrow> bool"
-where
-  "heap_invs s heap \<equiv> nodesValid s (ptr_coerce heap)"
-
+  where
+    "heap_invs s heap \<equiv> nodesValid s (ptr_coerce heap)"
+    
 lemma nodesValid_nodeValid: "nodesValid s n \<Longrightarrow> nodeValid s n"
   apply(subst (asm) nodesValid_def') unfolding Let_def by auto
-
+    
 lemma nodesValid_not_null:
   "nodesValid s heap \<Longrightarrow> heap \<noteq> NULL"
   by (meson c_guard_NULL_simp nodeValid_def nodesValid_def') 
-      
+    
 lemma heap_invs_not_null :"heap_invs s heap \<Longrightarrow> heap \<noteq> NULL" 
   unfolding heap_invs_def
   apply (drule nodesValid_not_null) by auto
-
+    
 lemma nodesValid_not_next_null:
   "nodesValid s node \<Longrightarrow> \<not> nodesValid s (node_next s node) \<Longrightarrow> (node_next s node) = NULL"
   using nodesValid.elims by auto 
-
+    
 lemma nodesValid_node_plus_1:
   "nodesValid s node \<Longrightarrow> node_next s node \<noteq> NULL \<Longrightarrow>
     (node +\<^sub>p 1) > node"
-sorry
-(* function reachable :: "globals \<Rightarrow> mem_node_C ptr \<Rightarrow> mem_node_C ptr \<Rightarrow> bool"
-where "reachable s node to = (let next = (node_next s node) in
-      if node = NULL then to = NULL 
-      else if node = to then True else (ptr_val next > ptr_val node \<and> reachable s next to))"
-by pat_completeness auto
-termination apply (relation "measure (\<lambda> (s,heap,n). unat (ptr_val n) - unat (ptr_val heap))")
-apply auto
-sorry *)
-  
+  sorry
+    
 function  reachable :: "globals \<Rightarrow> mem_node_C ptr \<Rightarrow> mem_node_C ptr \<Rightarrow> bool"
   where "reachable s NULL to = (to = NULL)"
   | "node \<noteq> NULL \<and> node = to \<Longrightarrow> reachable s node to = True"
@@ -180,34 +197,41 @@ function  reachable :: "globals \<Rightarrow> mem_node_C ptr \<Rightarrow> mem_n
      reachable s node to = (reachable s (node_next s node) to)"
   | "node \<noteq> NULL \<and> node \<noteq> to \<and> (node_next s node) = NULL  \<Longrightarrow>
      reachable s node to = (to = NULL)"
-    by (auto simp: ptr_less_simp ptr_le_simp) fastforce
+  by (auto simp: ptr_less_simp ptr_le_simp) fastforce
 termination
-  apply (relation "measure (\<lambda> (s,node,to).2 ^ 32 + unat (ptr_val to) - unat (ptr_val node))")
+  apply (relation "measure (\<lambda> (s,node,to).2 ^ 32 + unat_ptr to - unat_ptr node)")
    apply (auto simp: ptr_less_simp ptr_le_simp)
   by unat_arith auto
     
 thm reachable.induct        
 thm reachable.simps
   
-(* declare reachable.simps[simp del] *)
+  (* declare reachable.simps[simp del] *)
   
 lemma self_reachable: "n \<noteq> NULL \<Longrightarrow> reachable s n n"
   by auto
-
+    
 lemma reachable_helper1[rule_format]: 
   "reachable s node to \<longrightarrow> node \<ge> (node_next s node) \<longrightarrow> to \<noteq> NULL \<longrightarrow> node = to"
   apply (rule_tac ?a0.0=s and ?a1.0=node and ?a2.0=to in reachable.induct)
       apply auto[3]
    apply (auto simp del:reachable.simps)
   by auto
-
+    
 lemma reachable_helper2[rule_format]: "reachable s node to \<longrightarrow> to \<noteq> NULL \<longrightarrow> node \<le> to"
   by (rule_tac ?a0.0=s and ?a1.0=node and ?a2.0=to in reachable.induct) auto
     
 lemma reachable_helper3[rule_format]:
   "reachable s node to \<longrightarrow> node_next s node = NULL \<longrightarrow> node \<noteq> to \<longrightarrow> to = NULL "
   by (rule_tac ?a0.0=s and ?a1.0=node and ?a2.0=to in reachable.induct) auto  
-
+    
+lemma reachable_next_le_to[rule_format]:
+  "reachable s node to \<longrightarrow> node \<noteq> to \<longrightarrow> to \<noteq> NULL \<longrightarrow> node_next s node \<le> to  "
+  apply (rule_tac ?a0.0=s and ?a1.0=node and ?a2.0=to in reachable.induct)
+      apply auto
+  using reachable_helper2 by blast
+    
+    
 lemma reachable_trans[rule_format]:
   "reachable s node to \<longrightarrow> to \<noteq> NULL \<longrightarrow> node_next s to > to \<longrightarrow> 
    reachable s node (node_next s to)"
@@ -221,29 +245,18 @@ lemma reachable_trans[rule_format]:
    apply (drule_tac node="node_next s (node_next s to)" in reachable_helper2)
     apply simp
   by (auto simp: ptr_le_simp ptr_less_simp)  
-  
+    
 lemma reachable_trans2[rule_format]:
   "reachable s node to \<longrightarrow> to \<noteq> NULL \<longrightarrow> node_next s to = NULL \<longrightarrow> 
    reachable s node (node_next s to)"
   apply (rule_tac ?a0.0=s and ?a1.0=node and ?a2.0=to in  reachable.induct)
   by auto
-
-(* FIXME remove this *)    
-function reachable_old :: "globals \<Rightarrow> mem_node_C ptr \<Rightarrow> mem_node_C ptr \<Rightarrow> bool"
-where "reachable_old s heap n = (heap \<noteq> NULL \<and>
-      (heap = n \<or> 
-       (\<exists> n'. n = (node_next s n') \<and>
-          ptr_val n > ptr_val n' \<and> reachable_old s heap n')))"
-by pat_completeness auto
-termination apply (relation "measure (\<lambda> (s,heap,n). unat (ptr_val n))")
-apply auto
-  oops
-
+    
 lemma updated_node_hrs_the_same_elsewhere_correct:
   assumes x_val:"x \<notin> ptr_span p"
   shows"hrs_the_same_at s (update_node s p new_node) x" 
-sorry
-  
+  sorry
+    
 lemma updated_node_hrs_the_same_elsewhere_incorrect :
   assumes x_val:"x \<ge> ptr_val (p +\<^sub>p 1) \<or> x < ptr_val p"
   shows"hrs_the_same_at s (update_node s p new_node) x" 
@@ -255,11 +268,11 @@ proof-
     hence "ptr_span p \<inter> {ptr_val ?xptr..+size_of TYPE(8 word)} = {}" 
       unfolding intvl_def apply simp unfolding ptr_add_def apply simp  sorry
   }
-    {assume "ptr_val ?xptr < ptr_val p"
+  {assume "ptr_val ?xptr < ptr_val p"
     hence "ptr_span p \<inter> {ptr_val ?xptr..+size_of TYPE(8 word)} = {}" 
       unfolding intvl_def apply simp unfolding ptr_add_def   sorry
   }
-     hence "ptr_span p \<inter> {ptr_val ?xptr..+size_of TYPE(8 word)} = {}" sorry (* oops *)
+  hence "ptr_span p \<inter> {ptr_val ?xptr..+size_of TYPE(8 word)} = {}" sorry (* oops *)
   hence "\<forall> h. h_val (heap_update p new_node h) ?xptr = h_val h ?xptr" 
     using h_val_update_regions_disjoint by blast
   hence "\<forall> h. (heap_update p new_node h)  x =  h x" 
@@ -274,22 +287,22 @@ proof-
 qed
 thm t_hrs_'_update_def
 thm t_hrs_'_def
-
+  
 lemma updated_node_blahblah:
   "x \<ge> ptr_val (p+\<^sub>p 1) \<and> x \<ge> ptr_val (q +\<^sub>p 1) \<Longrightarrow> 
     hrs_the_same_at s (update_node (update_node s p new_node_1) q new_node_2 ) x"
   (* FIXME error *)
-using updated_node_hrs_the_same_elsewhere
-by presburger
-
+  using updated_node_hrs_the_same_elsewhere
+  by presburger
+    
 lemma updated_node_blahblah_2:
   "x < ptr_val p \<and> x < ptr_val q \<Longrightarrow> 
     hrs_the_same_at s (update_node (update_node s p new_node_1) q new_node_2 ) x"
-   (* FIXME error *)
-using updated_node_hrs_the_same_elsewhere
-by presburger  
-
-  
+  (* FIXME error *)
+  using updated_node_hrs_the_same_elsewhere
+  by presburger  
+    
+    
 function path :: "globals \<Rightarrow> mem_node_C ptr \<Rightarrow> mem_node_C ptr \<Rightarrow> mem_node_C ptr list"
   where "node = NULL \<or> node \<ge> node_next s node \<or> node_next s node > to \<Longrightarrow>
           path s node to = []"
@@ -300,10 +313,10 @@ function path :: "globals \<Rightarrow> mem_node_C ptr \<Rightarrow> mem_node_C 
      apply auto 
   by (metis  dual_order.strict_iff_order le_cases)
 termination
-  apply (relation "measure (\<lambda> (s,node,to).2 ^ 32 + unat (ptr_val to) - unat (ptr_val node))")
+  apply (relation "measure (\<lambda> (s,node,to).2 ^ 32 + unat_ptr to - unat_ptr node)")
    apply (auto simp:ptr_less_simp ptr_le_simp)
   by unat_arith     
-
+    
 lemma path_not_empty_node_cond[rule_format]: "set (path s node to) \<noteq> {} \<longrightarrow> 
         node \<noteq> NULL \<and>
         ptr_val node < ptr_val (node_next s node) \<and>
@@ -316,7 +329,7 @@ lemma path_not_empty_node_cond[rule_format]: "set (path s node to) \<noteq> {} \
     
 lemma p_in_path_not_in_next_eq : 
   assumes p_in_path: "p \<in> set (path s node to)" 
-      and p_not_in_next: "p \<notin> set (path s (node_next s node) to)" 
+    and p_not_in_next: "p \<notin> set (path s (node_next s node) to)" 
   shows "p = node"
 proof-
   from p_in_path have " (path s node to) = node # (path s (node_next s node) to)"
@@ -328,29 +341,80 @@ proof-
 qed
   
 lemma p_in_path_l_to[rule_format]:  
-   " p \<in> set (path s node to ) \<longrightarrow> p < to"
+  " p \<in> set (path s node to ) \<longrightarrow> p < to"
   apply (rule_tac ?P = "\<lambda> s node to. p \<in> set (path s node to ) \<longrightarrow> p < to" in path.induct)
   by auto
     
 lemma p_in_path_ge_node[rule_format]:
- "p \<in> set (path s node to) \<longrightarrow> p \<ge> node"
- apply (rule_tac ?a0.0=s and ?a1.0=node and ?a2.0=to in path.induct)
+  "p \<in> set (path s node to) \<longrightarrow> p \<ge> node"
+  apply (rule_tac ?a0.0=s and ?a1.0=node and ?a2.0=to in path.induct)
   by auto
     
 lemma p_in_path_next_le_to[rule_format]:
   "p \<in> set (path s node to) \<longrightarrow> (node_next s p) \<le> to"
   apply (rule_tac ?a0.0=s and ?a1.0=node and ?a2.0=to in path.induct)
-by auto
-
+  by auto
+    
+lemma p_in_path_l_next[rule_format]:
+  "p \<in> set (path s node to) \<longrightarrow> node < (node_next s p)"
+  apply (rule_tac ?a0.0=s and ?a1.0=node and ?a2.0=to in path.induct)
+  by auto
+    
 lemma heaps_eq_imp_paths_eq:
   "\<forall> p . p \<ge> ptr_val fst_node \<and> p < ptr_val to \<longrightarrow> hrs_the_same_at  s s' p
        \<Longrightarrow>  path s fst_node to = path s' fst_node to" 
-apply (induction rule:path.induct)  
+  apply (induction rule:path.induct)  
   sorry
     
+lemma nodeValid_edge_of_addr_space:
+  assumes "nodeValid s node"
+  shows "(node +\<^sub>p 1) > node \<or> (node_size_masked s node) = 0"
+  unfolding nodeValid_def
+proof -
+  have "unat (node_size_masked s node) * 8 < 2 ^ LENGTH(32)" using `nodeValid s node`
+    unfolding nodeValid_def by meson
+  hence "unat (node_size_masked s node) * 8 = unat ((node_size_masked s node) * 8)"
+    using unat_mult_lem  by (metis sable_isa.eight_eq_eight)
+  {assume "(node_size_masked s node) \<noteq> 0"    
+    hence "(node_size_masked s node) * 8 \<noteq> 0"
+      using `unat (node_size_masked s node) * 8 = unat ((node_size_masked s node) * 8)`
+      using unat_eq_zero by fastforce
+    hence "unat_ptr node + 8 < 2 ^ LENGTH(32)" 
+      using `nodeValid s node` apply simp
+      apply (frule nodeValid_node_size_l1_new) 
+      apply auto
+      by (meson add_le_same_cancel1 le_def less_le_trans not_gr_zero unat_eq_zero) 
+    hence "(node +\<^sub>p 1) > node" 
+      unfolding ptr_add_def 
+      apply (simp add:ptr_less_simp)
+      by unat_arith auto
+  } thus ?thesis by fast
+qed
+  
+lemma intvl_no_overflow_lower_bound:
+  "(a :: ('a::{len}) word) \<in> {x ..+  sz} \<Longrightarrow> unat x + sz \<le> 2 ^ LENGTH('a) \<Longrightarrow> a \<ge> x"
+  apply unat_arith unfolding intvl_def  apply unat_arith
+  apply auto 
+  apply (subgoal_tac "unat (of_nat k) = k")
+   apply (smt add.commute add_leD1 add_less_mono1 order_less_le_trans unat_of_nat unat_of_nat_eq word_nchotomy)
+  by (smt add.commute add.left_neutral add_diff_cancel_right' add_leD1 add_lessD1 diff_add_inverse diff_diff_cancel diff_le_self le_Suc_ex less_diff_conv less_irrefl_nat less_or_eq_imp_le linorder_not_less nat_add_left_cancel_less nat_less_le not_add_less1 order_less_le_trans unat_of_nat_eq)
+    
+lemma intvl_upper_bound: "a \<in> {x ..+ sz} \<Longrightarrow> 
+  unat a < unat x + sz"
+  unfolding intvl_def
+  apply unat_arith
+  apply (auto simp add: unat_of_nat) 
+  using mod_less by blast
+    
+    (* thm zero_not_in_intvl_no_overflow[THEN intvl_no_overflow_lower_bound] *)
+lemma zero_not_in_intvl_lower_bound:
+  "(a::('a::len) word) \<in> {x ..+ sz} \<Longrightarrow> 0 \<notin> {x ..+  sz}  \<Longrightarrow> a \<ge>  x "
+  apply (drule zero_not_in_intvl_no_overflow)
+  by (rule intvl_no_overflow_lower_bound)
+    
 lemma hrs_the_same_imp_nodeValid:
-  "\<forall>p \<in> {ptr_val node ..+ size_of (TYPE(mem_node_C))}. hrs_the_same_at s s' p \<Longrightarrow>
-   \<forall>p \<in> {ptr_val (node +\<^sub>p 1) ..+ unat (node_size_masked s node) * size_of TYPE(mem_node_C)}. hrs_the_same_at s s' p \<Longrightarrow>   
+  "\<forall> p \<in> ptr_span node. hrs_the_same_at s s' p \<Longrightarrow>
+   \<forall> p \<in> array_span (node +\<^sub>p 1) (unat (node_size_masked s node)). hrs_the_same_at s s' p \<Longrightarrow>   
    nodeValid s node \<Longrightarrow> 
    nodeValid s' node"
   unfolding nodeValid_def nodeFree_def Let_def
@@ -364,21 +428,65 @@ lemma hrs_the_same_imp_nodeValid:
   apply (frule hrs_the_same_nodes_the_same) apply auto[1]
   done
     
+lemma hrs_the_same_imp_nodeValid2:
+  assumes hrs_the_same:"\<forall> p . p\<ge> ptr_val node \<and> unat p < unat_ptr node + 8 + (unat (node_size_masked s node)) * 8 \<longrightarrow>
+    hrs_the_same_at s s' p"
+    and "nodeValid s node"
+  shows "nodeValid s' node"
+proof-
+  have 1:"\<forall> p \<in> ptr_span node. p \<ge> ptr_val node" using `nodeValid s node`
+    apply auto
+    unfolding nodeValid_def c_guard_def c_null_guard_def
+    apply (rule intvl_no_overflow_lower_bound)
+     apply auto[1] 
+    by (metis mem_node_C_size zero_not_in_intvl_no_overflow)     
+  have "\<forall> p \<in> ptr_span node. unat p <unat_ptr node + 8" 
+    using sable_isa.intvl_upper_bound by auto
+  hence "\<forall> p \<in> ptr_span node. unat p <unat_ptr node + 8 + (unat (node_size_masked s node)) * 8"
+    by auto
+  with 1 have c1:"\<forall> p \<in> ptr_span node. hrs_the_same_at s s' p" 
+    using hrs_the_same by simp
+      
+  let ?arr_span = "array_span (node +\<^sub>p 1) (unat (node_size_masked s node))"  
+  have "(node +\<^sub>p 1) > node \<or> (node_size_masked s node) = 0"
+    using `nodeValid s node` nodeValid_edge_of_addr_space by simp
+  moreover {
+    assume "(node +\<^sub>p 1) > node"  
+    have "\<forall>p \<in> ?arr_span . p \<ge> ptr_val node"
+      apply auto
+      apply (frule intvl_no_overflow_lower_bound)
+      using `nodeValid s node`
+      using sable_isa.nodeValid_node_size_l2 apply blast
+      using `(node +\<^sub>p 1) > node`
+      by (meson le_less_trans less_irrefl nat_le_linear ptr_less_def ptr_less_def' word_le_nat_alt)
+    moreover have "\<forall>p \<in> ?arr_span.unat p < unat_ptr node + 8 + (unat (node_size_masked s node)) * 8"
+      apply auto
+      apply (drule intvl_upper_bound) 
+      unfolding ptr_add_def
+      by unat_arith
+    ultimately have "\<forall>p \<in> ?arr_span. hrs_the_same_at s s' p" 
+      using hrs_the_same by simp
+  }
+  moreover{
+    assume "(node_size_masked s node) = 0"
+    hence "?arr_span = {}" by simp
+    hence "\<forall> p \<in> ?arr_span. hrs_the_same_at s s' p" by blast
+  }
+  ultimately have "\<forall> p \<in> ?arr_span. hrs_the_same_at s s' p" by argo
+  with `nodeValid s node` c1 show ?thesis
+    using hrs_the_same_imp_nodeValid by presburger
+qed
+  
 lemma nodeValid_imp_range_l:
   "ptr_val n < ptr_val to \<Longrightarrow> nodeValid s n \<Longrightarrow> nodeValid s to \<Longrightarrow> 
-      \<forall> p \<in>{ptr_val n ..+ size_of (TYPE(mem_node_C))}. p < ptr_val to"
+      \<forall> p \<in> ptr_span n. p < ptr_val to"
   sorry
     
-lemma "nodesValid s heap \<Longrightarrow>
-       \<forall> p . p \<ge> ptr_val heap \<and> p < ptr_val (last_node +\<^sub>p 1) \<longrightarrow>  hrs_the_same_at s s' p
-       \<Longrightarrow> \<forall> n \<in> set (path s heap last_node). nodeValid s' n"
-  sorry
-          
 lemma nodesValid_trans_back: "nodeValid s node \<Longrightarrow> 
     nodesValid s (node_next s node) \<Longrightarrow>
     nodesValid s node"
   by(subst nodesValid_def', simp)
-
+    
 thm nodesValid.induct[simplified]
 lemma nodesValid_reachable_imp_nodesValid: 
   "reachable s fst_node node \<Longrightarrow>
@@ -439,33 +547,33 @@ proof-
       by presburger
   } moreover{ assume "node_next s node = NULL"
     hence "reachable s fst_node (node_next s node)" using reachable `node \<noteq> NULL` 
-      reachable_trans2 by presburger
+        reachable_trans2 by presburger
   }
   ultimately show "reachable s fst_node (node_next s node)" by argo
 qed      
-
+  
 lemma nodesValid_reachable_imp_nodeValid: "nodesValid s heap \<Longrightarrow> reachable s  heap node
       \<Longrightarrow> node \<noteq> NULL \<Longrightarrow> nodeValid s node"
   apply (drule nodesValid_reachable_imp_nodesValid)
   by assumption+ (meson nodesValid_def')
     
 thm word_mult_le_mono1
-
+  
 lemma l10: "unat x + unat y < 2 ^ 32 \<Longrightarrow>y \<noteq> 0 \<Longrightarrow> 
             ((x:: word32) div ( y :: word32)) * y + y \<ge> x"
   apply (subgoal_tac "unat (x div y * y) = (unat x div unat y) * unat y")
-
-sorry
-
+    
+  sorry
+    
 lemma l11:"((x::word32) || (scast (y::  32 signed word))) && (scast (~~y)) = x && (scast (~~y))"
-apply (subst word_ao_dist)
+  apply (subst word_ao_dist)
 proof -
   have " ((scast y)::word32) && scast (~~ y) = 0" unfolding scast_def sorry
   hence " x && scast (~~ y) || scast y && scast (~~ y) = x && scast (~~ y) || 0"
     by (simp add: \<open>scast y && scast (~~ y) = 0\<close>)
   thus "x && scast (~~ y) || scast y && scast (~~ y) = x && scast (~~ y)"  by simp
 qed
-
+  
 lemma mask_sw32_eq_0_eq_x :
   assumes "(x::word32) && scast (flag:: 32 signed word) = 0"
   shows " x && scast (~~flag) = x"
@@ -475,15 +583,16 @@ proof -
   have l1[simp]: "?neg_flag_w32 = ~~ ?flag_w32" sorry
   thus ?thesis using assms by (simp add: mask_eq_0_eq_x)
 qed
-
-(* declare [[show_types]]  *)
-(* declare [[show_sorts]] *)
-(* declare [[show_consts]] *)
+  
+  (* declare [[show_types]]  *)
+  (* declare [[show_sorts]] *)
+  (* declare [[show_consts]] *)
   
 lemma hrs_the_sam_nodesValid_reachable_imp_reachable:
   assumes "reachable s heap node"
     and "nodesValid s heap"
     and "\<forall>p . p \<ge> ptr_val heap \<and> p < ptr_val node \<longrightarrow> hrs_the_same_at s s' p"
+    and "node \<noteq> NULL"
   shows "reachable s' heap node" 
   sorry
     
@@ -496,17 +605,12 @@ lemma node_in_path_nodesValid_imp_nodeValid_node[rule_format]:
     apply (erule nodesValid_nodeValid)+
   apply (frule nodesValid_not_next_null)
   by auto
-
-thm path.simps
-thm nodeValid_def 
-thm path.simps(2)
-thm reachable.simps
-  
+    
 lemma nodesValid_reachable_imp_in_path: 
   assumes nodesValid: "nodesValid s fst_node" 
-  and reachable:"reachable s fst_node to"
-  and "to \<noteq> NULL" and "fst_node \<noteq> to"
-shows  "fst_node \<in> set (path s fst_node to)"
+    and reachable:"reachable s fst_node to"
+    and "to \<noteq> NULL" and "fst_node \<noteq> to"
+  shows  "fst_node \<in> set (path s fst_node to)"
 proof-
   let ?next = "node_next s fst_node"
   from nodesValid have "nodeValid s fst_node" using nodesValid_def' by meson
@@ -518,14 +622,14 @@ proof-
   have "fst_node \<noteq> NULL" using `c_guard fst_node` by force
   have "reachable s ?next to" 
     using `fst_node < ?next` `fst_node \<noteq> NULL` `fst_node \<noteq> to` reachable
-    reachable.simps(4) by simp
+      reachable.simps(4) by simp
   hence "?next \<le> to" using `to \<noteq> NULL` by (rule reachable_helper2) 
   hence "path s fst_node to = fst_node # path s ?next to" 
     using `fst_node \<noteq> NULL` `fst_node < ?next` `?next \<le> to`    
-    path.simps(2) by fast
+      path.simps(2) by fast
   thus ?thesis by simp
 qed
-
+  
 lemma node_reachable_in_path[rule_format]:
   "reachable s node to \<longrightarrow> node \<noteq> to\<longrightarrow> to \<noteq> NULL \<longrightarrow> node \<in> set (path s node to )"
   apply(rule_tac ?a0.0=s and ?a1.0=node and ?a2.0=to in reachable.induct)
@@ -534,40 +638,6 @@ lemma node_reachable_in_path[rule_format]:
    apply (frule path_not_empty_node_cond)
    apply (subgoal_tac "(node_next s node) \<le> to")
   by (auto simp:ptr_le_simp ptr_less_simp)
-    
-lemma nodeValid_edge_of_addr_space:
-  assumes "nodeValid s node"
-    shows "(node +\<^sub>p 1) > node \<or> (node_size_masked s node) = 0"
-  unfolding nodeValid_def
-proof -
-  have "unat (node_size_masked s node) * 8 < 2 ^ LENGTH(32)" using `nodeValid s node`
-    unfolding nodeValid_def by meson
-  hence "unat (node_size_masked s node) * 8 = unat ((node_size_masked s node) * 8)"
-    using unat_mult_lem  by (metis sable_isa.eight_eq_eight)
-  {assume "(node_size_masked s node) \<noteq> 0"    
-    hence "(node_size_masked s node) * 8 \<noteq> 0"
-      using `unat (node_size_masked s node) * 8 = unat ((node_size_masked s node) * 8)`
-      using unat_eq_zero by fastforce
-    hence "unat (ptr_val node) + 8 < 2 ^ LENGTH(32)" 
-      using `nodeValid s node` apply simp
-      apply (frule nodeValid_node_size_l1_new) 
-      apply auto
-      by (meson add_le_same_cancel1 le_def less_le_trans not_gr_zero unat_eq_zero) 
-    hence "(node +\<^sub>p 1) > node" 
-      unfolding ptr_add_def 
-      apply (simp add:ptr_less_simp)
-      by unat_arith auto
-  } thus ?thesis by fast
-qed
-  
-lemma intvl_no_overflow_lower_bound:
-  "(a :: 32 word) \<in> {x ..+  sz} \<Longrightarrow> unat x + sz \<le> 2 ^ LENGTH(32) \<Longrightarrow> a \<ge> x"
-  apply unat_arith unfolding intvl_def  apply unat_arith
-  apply auto 
-  apply (subgoal_tac "unat (of_nat k) = k")
-   apply (smt Divides.mod_less_eq_dividend add.commute add_diff_cancel_right' le_less_trans len_of_addr_card less_diff_conv unat_of_nat)
-  apply(rule unat_of_nat32') 
-  by simp
     
 lemma nodeValid_heaps_eq_imp_nodeValid:
   assumes "nodeValid s node"
@@ -580,7 +650,7 @@ proof-
     unfolding nodeValid_def by meson
   hence "unat ?node_size * 8 = unat (?node_size * 8)"
     using unat_mult_lem  by (metis sable_isa.eight_eq_eight)
-  have 0:"unat (ptr_val (node +\<^sub>p 1)) + unat (?node_size * 8) \<le>  2 ^ LENGTH(32)"
+  have 0:"unat_ptr (node +\<^sub>p 1) + unat (?node_size * 8) \<le>  2 ^ LENGTH(32)"
     using `nodeValid s node` by (rule nodeValid_node_size_l1)      
   have "\<forall> p \<in> ptr_span node. p \<ge> ptr_val node" 
     using `c_guard node` unfolding c_guard_def c_null_guard_def
@@ -623,36 +693,36 @@ lemma nodesValid_heaps_eq_imp_nodesValid[rule_format]:
     apply auto[1]
    defer
    apply clarify
-    defer
+   defer
 proof clarify
   fix s heap
   assume "nodeValid s heap"
-       "node_next s heap = NULL"
-       "nodesValid s heap"
-       and hrs_the_same:"\<forall>x\<ge>ptr_val heap. hrs_the_same_at s s' x"  
+    "node_next s heap = NULL"
+    "nodesValid s heap"
+    and hrs_the_same:"\<forall>x\<ge>ptr_val heap. hrs_the_same_at s s' x"  
   have "c_guard heap" using `nodeValid s heap` unfolding nodeValid_def by meson
   hence "\<forall> p \<in> ptr_span heap. p \<ge> ptr_val heap" 
-     unfolding c_guard_def c_null_guard_def
+    unfolding c_guard_def c_null_guard_def
     apply auto
     apply (drule zero_not_in_intvl_no_overflow)
     apply (erule intvl_no_overflow_lower_bound) by assumption
   hence "\<forall> p \<in> ptr_span heap. hrs_the_same_at s s' p" using hrs_the_same by blast
   hence "node_val s heap = node_val s' heap" using hrs_the_same_nodes_the_same by blast     
   hence "node_next s' heap = NULL" using `node_next s heap = NULL` by argo
-  
+      
   have "nodeValid s' heap" using `nodeValid s heap` hrs_the_same 
     using nodeValid_heaps_eq_imp_nodeValid by blast
   show "nodesValid s' heap" using `node_next s' heap = NULL` `nodeValid s' heap`
-       by auto
+    by auto
 next 
   fix s heap
   assume ih: "nodesValid s (node_next s heap) \<longrightarrow>
           (\<forall>x\<ge>ptr_val (node_next s heap).hrs_the_same_at s s' x) \<longrightarrow>
           nodesValid s' (node_next s heap)"
-       and "nodeValid s heap"
-       and "node_next s heap \<noteq> NULL"
-       and "nodesValid s heap"
-       and hrs_the_same:"\<forall>x\<ge>ptr_val heap. hrs_the_same_at s s' x"
+    and "nodeValid s heap"
+    and "node_next s heap \<noteq> NULL"
+    and "nodesValid s heap"
+    and hrs_the_same:"\<forall>x\<ge>ptr_val heap. hrs_the_same_at s s' x"
   have "c_guard heap" using `nodeValid s heap` unfolding nodeValid_def by meson
   have "\<forall>p \<in> ptr_span heap. hrs_the_same_at s s' p" using `c_guard heap` hrs_the_same
     unfolding c_guard_def c_null_guard_def
@@ -673,20 +743,11 @@ next
   moreover have "nodeValid s' heap" using hrs_the_same `nodeValid s heap` 
     using nodeValid_heaps_eq_imp_nodeValid by blast
   ultimately show "nodesValid s' heap" using nodesValid_trans_back by fast
-qed
+qed 
   
-thm nodesValid.simps  
-lemma nodesValid_l1:
-assumes "nodesValid s node" 
-    and "nodeValid s' node"
-    and "c_guard (node +\<^sub>p 1)"
-    and "\<forall>x. x \<ge> ptr_val (node +\<^sub>p 1) \<longrightarrow> hrs_the_same_at s s' x"
-shows "nodesValid s' node"
-  sorry
-
 thm nodesValid_reachable_imp_in_path
-lemma nodesValid_l2[rule_format]:
-      "nodeValid s heap \<longrightarrow>
+lemma path_nodeValid_reachable_imp_nodesValid[rule_format]:
+  "nodeValid s heap \<longrightarrow>
        (\<forall> p \<in> set (path s heap node). nodeValid s p) \<longrightarrow>
        reachable s heap node \<longrightarrow>
        nodesValid s node \<longrightarrow>
@@ -705,8 +766,6 @@ lemma nodesValid_l2[rule_format]:
   apply auto
    apply (frule node_reachable_in_path)
      apply auto
-     (* FIXME error *)
-    apply (frule nodesValid_nodeValid, auto)
    apply (frule nodesValid_not_null, auto)
   using sable_isa.nodesValid_def' unfolding Let_def by blast
     
@@ -715,13 +774,13 @@ lemma nodesValid_l3:
    node_next s node = NULL \<Longrightarrow>
     nodesValid s node"
   by (meson nodesValid_def')
-  
+    
 lemma c_guard_l1:
   assumes "c_guard (a::('a::mem_type) ptr)"
-  "\<not> c_guard (a +\<^sub>p 1)"
-  "b > a" 
-  "b \<ge> a +\<^sub>p 1"
-shows "\<not> c_null_guard b" 
+    "\<not> c_guard (a +\<^sub>p 1)"
+    "b > a" 
+    "b \<ge> a +\<^sub>p 1"
+  shows "\<not> c_null_guard b" 
 proof -
   have "\<not> c_null_guard ( a +\<^sub>p 1)" using `c_guard a` `\<not> c_guard (a +\<^sub>p 1)`
     unfolding c_guard_def apply auto    
@@ -730,7 +789,7 @@ proof -
   have "0 \<in> ptr_span b" using `b \<ge> a +\<^sub>p 1` using `0 \<in> ptr_span (a +\<^sub>p 1)` unfolding intvl_def
   proof simp
     assume "a +\<^sub>p 1 \<le> b"
-       and "\<exists>k. ptr_val (a +\<^sub>p 1) + of_nat k = 0 \<and> k < size_of TYPE('a)"
+      and "\<exists>k. ptr_val (a +\<^sub>p 1) + of_nat k = 0 \<and> k < size_of TYPE('a)"
     then obtain k where k:"ptr_val (a +\<^sub>p 1) + of_nat k = 0 \<and> k < size_of TYPE('a)" by auto
     hence "ptr_val (a +\<^sub>p 1) + of_nat k = 0" by auto
     {
@@ -763,17 +822,17 @@ proof -
       let ?k2' = "of_nat (size_of TYPE('a)) - ( ptr_val b - ptr_val a)"
       have "ptr_val b > ptr_val a" using `b>a` 
         by (simp add: ptr_less_def ptr_less_def')
-      hence "unat (ptr_val b) > unat (ptr_val a)" using unat_mono by auto
+      hence "unat_ptr b > unat_ptr a" using unat_mono by auto
       from k_eq_0 have "ptr_val (a +\<^sub>p 1)= 0" using k by unat_arith
       hence 1:"ptr_val a + of_nat (size_of TYPE('a)) = 0" unfolding ptr_add_def by simp
       hence 2: "ptr_val b - ptr_val a < of_nat (size_of TYPE('a))" 
         using k_eq_0
         apply unat_arith (* SLOW! *) apply auto
-         apply (subgoal_tac "unat (ptr_val a) \<noteq> (0::nat)")
+         apply (subgoal_tac "unat_ptr a \<noteq> (0::nat)")
           apply auto[1]
         using `c_guard a` 
          apply (metis len_of_addr_card max_size mem_type_simps(3) neq0_conv unat_of_nat_len)
-        using `unat (ptr_val b) > unat (ptr_val a)` by simp
+        using `unat_ptr b > unat_ptr a` by simp
       hence "ptr_val b + ?k2' = 0" using 1  by (simp add: add.commute)
       hence 3:"ptr_val b + of_nat (unat ?k2') = 0" by simp
       have "ptr_val b - ptr_val a > 0" using `ptr_val b > ptr_val a` 
@@ -788,9 +847,102 @@ proof -
   qed 
   thus "\<not> c_null_guard b" unfolding c_null_guard_def by auto
 qed
-
+  
 lemma self_impl: "Q \<Longrightarrow> Q" by assumption
-
+    
+lemma nodeValid_next_val: "nodeValid s node \<Longrightarrow>
+  node_next s node \<noteq> NULL \<Longrightarrow>
+  unat_ptr (node_next s node) \<ge> unat_ptr node + 8 +  unat ((node_size_masked s node) * 8)"
+  unfolding nodeValid_def Let_def 
+  by(simp split:if_split) 
+    
+    (* FIXME put somewhere else *)    
+lemma unat_add_lem_3:
+  "unat (a::'a::len word) + unat b + unat c < 2 ^ LENGTH('a) =
+    (unat (a + b + c) = unat a + unat b + unat c)"
+  using unat_add_lem
+  by (metis add_lessD1 unat_lt2p) 
+    
+    (* consider adding more to the conclusion *)
+lemma nodesValid_heaps_eq_nodeValid_in_path: 
+  assumes "nodesValid s heap"
+    and hrs_the_same: "\<forall> p . p \<ge> ptr_val heap \<and> p < ptr_val to \<longrightarrow> hrs_the_same_at s s' p"
+    and "reachable s heap to"
+    and "to \<noteq> NULL"
+  shows "\<forall> n \<in> set (path s' heap to). nodeValid s' n"
+proof-  
+  have "path s heap to = path s' heap to" using hrs_the_same 
+    using heaps_eq_imp_paths_eq by blast
+  { fix n
+    assume n_in_path_s':"n \<in> set (path s' heap to)"    
+    hence n_in_path:"n \<in> set (path s heap to)" using `path s heap to = path s' heap to`
+      by argo
+    have "n \<ge> heap" using n_in_path 
+      using p_in_path_ge_node by blast
+    have "nodeValid s n" using n_in_path `nodesValid s heap` 
+      using node_in_path_nodesValid_imp_nodeValid_node by blast
+    have c1:"\<forall> p . p\<ge> ptr_val n \<longrightarrow> p \<ge> ptr_val heap" using `n \<ge> heap` 
+      apply(simp add: ptr_le_simp) 
+      by fastforce
+    have "node_next s n \<noteq> NULL" using n_in_path
+      apply auto
+      apply(drule p_in_path_l_next) 
+      by (simp add: ptr_less_def ptr_less_def')
+    hence "unat_ptr n + 8 + unat ((node_size_masked s n) * 8) \<le> unat_ptr (node_next s n)"
+      using `nodeValid s n` sable_isa.nodeValid_next_val by blast
+    moreover have "node_next s n \<le> to" using n_in_path 
+      using p_in_path_next_le_to by fast
+    ultimately have "unat_ptr n + 8 + unat ((node_size_masked s n) * 8) \<le> unat_ptr to"
+      apply(auto simp:ptr_le_simp) by unat_arith 
+    hence "unat_ptr n + 8 + unat (node_size_masked s n) * 8 \<le> unat_ptr to"     
+      apply unat_arith apply auto 
+      by (metis \<open>nodeValid s n\<close> nodeValid_def sable_isa.eight_eq_eight unat_of_nat_eq word_arith_nat_mult)
+    hence c2:"\<forall> p . unat p < unat_ptr n + 8 + (unat (node_size_masked s n)) * 8
+      \<longrightarrow> p <ptr_val to" apply auto 
+      using less_le_trans word_less_nat_alt by blast     
+    have "\<forall> p . p\<ge> ptr_val n \<and> unat p < unat_ptr n + 8 + (unat (node_size_masked s n)) * 8 \<longrightarrow>
+      hrs_the_same_at s s' p" using c1 c2
+      using hrs_the_same by presburger
+    with `nodeValid s n` have "nodeValid s' n" 
+      using hrs_the_same_imp_nodeValid2 by presburger
+  }
+  thus ?thesis by fast
+qed
+  
+  (*FIXME move these out of here  *) 
+  
+lemma OCC_FLAG_helper1: "(x::32 word) && (scast OCC_FLG) = 0 \<Longrightarrow>
+    y \<le> x \<Longrightarrow>
+    y && (scast OCC_FLG) = 0"
+  apply(subgoal_tac "scast OCC_FLG = ~~ ((mask 31)::32 word)")
+   apply(subgoal_tac "y && mask 31 = y ")
+    apply (frule mask_eq_x_eq_0[THEN iffD1])
+    apply simp
+   apply (subgoal_tac "x \<le> mask 31")
+    apply (metis (no_types, hide_lams) and_mask_eq_iff_le_mask less_le_trans not_less)
+   apply (metis add.left_neutral word_and_le1 word_bool_alg.double_compl word_plus_and_or_coroll2)
+  unfolding MEM_NODE_OCCUPIED_FLAG_def mask_def
+  by simp
+    
+lemma OCC_FLG_neg : "(scast (~~ MEM_NODE_OCCUPIED_FLAG) ::32 word) = ~~ scast MEM_NODE_OCCUPIED_FLAG"
+  by (metis (no_types) mask_eq_0_eq_x l11 mask_sw32_eq_0_eq_x word_bw_comms(1) word_log_esimps(7) 
+      word_log_esimps(9) word_not_not)
+    
+lemma unat_addition_less_pres:"unat (a::'a::len word) + unat b < unat c \<Longrightarrow> a + b < c"
+  by unat_arith
+lemma unat_addition_le_pres:"unat (a::'a::len word) + unat b \<le> unat c \<Longrightarrow> a + b \<le> c"
+  by unat_arith
+lemma shiftr3_upper_bound:"(x :: 32 word) >> 3 \<le> 0x1FFFFFFF"
+  apply (simp add:shiftr3_is_div_8)
+  apply unat_arith
+  by auto
+thm intvl_no_overflow   
+lemma intvl_no_overflow2:
+  "unat (a::'a::len word) + b \<le> 2 ^ LENGTH('a) \<Longrightarrow>
+(x \<in> {a..+b}) = (a \<le> x \<and> unat x < unat a + b)"
+  sorry
+thm intvl_no_overflow2[THEN iffD1]
+  
 lemma alloc'_invs:
   fixes size_bytes:: "32 word" and heap:: "unit ptr"
   assumes size_bytes_g0 : "size_bytes > 0"
@@ -800,8 +952,8 @@ lemma alloc'_invs:
   apply (subst whileLoop_add_inv 
       [where I="\<lambda> (n,r) s. heap_invs s heap \<and> reachable s (ptr_coerce heap) n
                   \<and> (r=0 \<longrightarrow> (n = NULL \<or> ((size_bytes >> 3) + 1
-                        \<le> size_C (h_val (hrs_mem (t_hrs_' s)) n) && scast (~~ MEM_NODE_OCCUPIED_FLAG))
-                     \<and> size_C (h_val (hrs_mem (t_hrs_' s)) n) && scast MEM_NODE_OCCUPIED_FLAG = 0))" 
+                        \<le> size_C (h_val (hrs_mem (t_hrs_' s)) n) && scast (~~ OCC_FLG))
+                     \<and> size_C (h_val (hrs_mem (t_hrs_' s)) n) && scast OCC_FLG = 0))" 
         and M="\<lambda> ((n,y),s). ptr_val n"])
   apply (wp )
       prefer 5
@@ -832,41 +984,45 @@ proof -
   fix a::"mem_node_C ptr"
   fix s::globals
   assume invs: "nodesValid s (ptr_coerce heap)"
-    and node_free :"node_size s a && scast MEM_NODE_OCCUPIED_FLAG = 0"
+    and node_free :"node_size s a && scast OCC_FLG = 0"
     and reachable: "reachable s (ptr_coerce heap) a"
     and "a \<noteq> NULL"
     and "c_guard a"
     (* and "c_guard (a +\<^sub>p uint (2 + (size_bytes >> 3))) " *)
+  let ?new_size_simplified = "(node_size s a && scast (~~ OCC_FLG) ||  scast OCC_FLG)"
+  let ?new_s = "(update_node s a (mem_node_C
+                (node_size s a && scast (~~ OCC_FLG) ||  scast OCC_FLG)
+                (node_next s a)))"
+  let ?new_size = "(node_size ?new_s a)"
+  let ?heap_node = "(ptr_coerce heap) :: mem_node_C ptr"
+  have "nodeValid s ?heap_node"  using `nodesValid s ?heap_node` 
+    using nodesValid_nodeValid by blast
+  hence "c_guard ?heap_node" unfolding nodeValid_def by metis
   from invs and reachable and `a \<noteq> NULL` have "nodesValid s a"
     using nodesValid_reachable_imp_nodesValid by simp
-  let ?new_size_simplified = "(node_size s a && scast (~~ MEM_NODE_OCCUPIED_FLAG) ||  scast MEM_NODE_OCCUPIED_FLAG)"
-  let ?new_s = "(update_node s a (mem_node_C
-                (node_size s a && scast (~~ MEM_NODE_OCCUPIED_FLAG) ||  scast MEM_NODE_OCCUPIED_FLAG)
-                (node_next s a)))"
-  let ?new_size = "(node_size ?new_s a) "
   have "node_next ?new_s a = node_next s a" using updated_node_next by auto
   have "?new_size = ?new_size_simplified" using updated_node_size by auto
-  have "?new_size_simplified  && scast (~~MEM_NODE_OCCUPIED_FLAG) =
-    node_size s a && scast (~~ MEM_NODE_OCCUPIED_FLAG) && scast (~~MEM_NODE_OCCUPIED_FLAG)"
+  have "?new_size_simplified  && scast (~~OCC_FLG) =
+    node_size s a && scast (~~ OCC_FLG) && scast (~~OCC_FLG)"
     using l11 by (simp add: word_bw_assocs(1))
-  hence "node_size s a && scast (~~ MEM_NODE_OCCUPIED_FLAG) =
-        ?new_size  && scast (~~MEM_NODE_OCCUPIED_FLAG)"
+  hence size_masked_the_eq:"node_size s a && scast (~~ OCC_FLG) =
+        ?new_size  && scast (~~OCC_FLG)"
     apply (subst `?new_size = ?new_size_simplified`) by simp
-  moreover have new_node_occupied: "?new_size_simplified && scast MEM_NODE_OCCUPIED_FLAG = scast MEM_NODE_OCCUPIED_FLAG"
+  moreover have new_node_occupied: "?new_size_simplified && scast OCC_FLG = scast OCC_FLG"
     unfolding MEM_NODE_OCCUPIED_FLAG_def using word_ao_absorbs(5) by blast
   moreover from invs and reachable and `a \<noteq> NULL` have "nodeValid s a" 
-      using nodesValid_reachable_imp_nodeValid by blast
-  moreover have "(?new_size && scast MEM_NODE_OCCUPIED_FLAG = (0::32 word) \<longrightarrow> nodeFree ?new_s a)" 
+    using nodesValid_reachable_imp_nodeValid by blast
+  moreover have "(?new_size && scast OCC_FLG = (0::32 word) \<longrightarrow> nodeFree ?new_s a)" 
     apply (simp add: `?new_size = ?new_size_simplified`)
     using MEM_NODE_OCCUPIED_FLAG_not_zero
     by (metis calculation(2) h_val_heap_update hrs_update(1) scast_0 scast_scast_id(2) size_C.size_C_def)
   moreover from `nodeValid s a` have "c_guard a \<and>
-       unat (ptr_val a) + 8 + unat ((?new_size && scast (~~MEM_NODE_OCCUPIED_FLAG)) * 8) 
-        \<le> ( if ((node_next ?new_s a) \<noteq> NULL) then unat (ptr_val (node_next ?new_s a)) else 2 ^ LENGTH(32)) 
-        \<and> unat (?new_size && scast (~~MEM_NODE_OCCUPIED_FLAG)) * 8 < 2 ^ LENGTH(32)" 
+       unat_ptr a + 8 + unat ((?new_size && scast (~~OCC_FLG)) * 8) 
+        \<le> ( if ((node_next ?new_s a) \<noteq> NULL) then unat_ptr (node_next ?new_s a) else 2 ^ LENGTH(32)) 
+        \<and> unat (?new_size && scast (~~OCC_FLG)) * 8 < 2 ^ LENGTH(32)" 
     unfolding nodeValid_def
-    apply (subst `node_size s a && scast (~~ MEM_NODE_OCCUPIED_FLAG) =
-        ?new_size  && scast (~~MEM_NODE_OCCUPIED_FLAG)`)
+    apply (subst `node_size s a && scast (~~ OCC_FLG) =
+        ?new_size  && scast (~~OCC_FLG)`)
     apply (subst ` node_next ?new_s a = node_next s a`)
     using calculation(1)
     by (metis next_C.next_C_def sable_isa.updated_node_val)       
@@ -877,74 +1033,156 @@ proof -
   moreover have hrs_the_same_after_a:
     "c_guard (a +\<^sub>p 1) \<Longrightarrow> \<forall> x. x \<ge> ptr_val (a +\<^sub>p 1) \<longrightarrow> hrs_the_same_at s ?new_s x"
     using updated_node_hrs_the_same_elsewhere_incorrect by simp
+  have next_eq:"node_next ?new_s a = node_next s a" using updated_node_next by fast
+      
+  have hrs_the_same_except_a:"\<forall>p. p \<notin> ptr_span a \<longrightarrow> hrs_the_same_at s ?new_s p"
+    using updated_node_hrs_the_same_elsewhere_correct by blast   
   {
-   assume "c_guard (a +\<^sub>p 1)"  
-   hence "nodesValid ?new_s a" 
-     using `nodesValid s a` `nodeValid ?new_s a` hrs_the_same_after_a nodesValid_l1 by blast
+    assume "node_next s a = NULL"
+    hence "node_next ?new_s a = NULL" using next_eq by presburger
+    hence "nodesValid ?new_s a" using `nodeValid ?new_s a` by simp
   } moreover {
-    assume "\<not> c_guard (a +\<^sub>p 1)"       
-    {
-      assume "node_next s a \<noteq> NULL" 
-      have "(node_next s a) > a" 
-        using `nodeValid s a` `node_next s a \<noteq> NULL` unfolding nodeValid_def by metis
-      moreover have "(node_next s a) \<ge> (a +\<^sub>p 1)" 
-        using `nodeValid s a` `node_next s a \<noteq> NULL` unfolding nodeValid_def by metis
-      ultimately have "\<not> c_null_guard (node_next s a)" 
-        using `c_guard a` `\<not> c_guard (a +\<^sub>p 1)` 
-        apply (rule_tac a=a and b="(node_next s a)" in c_guard_l1) by auto
-      from `nodesValid s a` `node_next s a \<noteq> NULL` have "nodeValid s (node_next s a)"
-        using nodesValid_def' unfolding nodeValid_def by metis
-      hence "c_guard (node_next s a)" unfolding nodeValid_def by meson
-      with `\<not> c_null_guard (node_next s a)` have False unfolding c_guard_def by auto
-    }
-    hence "node_next s a = NULL" by auto
-    hence "node_next ?new_s a = NULL" using `node_next ?new_s a = node_next s a` by auto
-    hence "nodesValid ?new_s a" using `nodeValid ?new_s a` nodesValid_l3 by blast
-    }
-    ultimately have "nodesValid ?new_s a"  by blast 
-    moreover have hrs_the_same_before_a: "\<forall> p. p< ptr_val a \<longrightarrow> hrs_the_same_at s ?new_s p" 
-      sorry
-    hence hrs_the_same_heap_to_a:"\<forall>p. p\<ge> ptr_val (ptr_coerce heap) \<and> p < ptr_val a \<longrightarrow> hrs_the_same_at s ?new_s p"
+    assume "node_next s a \<noteq> NULL"
+    hence "node_next s a > a" using `nodeValid s a` unfolding nodeValid_def by meson
+    have "nodesValid s (node_next s a)" 
+      using `nodesValid s a` `node_next s a \<noteq> NULL`
+      using nodesValid.simps by blast
+    have "node_next s a \<ge> (a +\<^sub>p 1)" using `nodeValid s a` `node_next s a \<noteq> NULL`
+      unfolding nodeValid_def by meson
+        
+    have "\<forall>p \<in> ptr_span a. unat p < unat_ptr a + 8" 
+      using intvl_upper_bound by auto
+    moreover from `nodeValid s a` `node_next s a \<noteq> NULL`
+    have "unat_ptr (node_next s a) \<ge> unat_ptr a + 8"
+      using `nodeValid s a` `node_next s a \<noteq> NULL` 
+      apply simp apply (frule nodeValid_next_val) by auto
+    ultimately have "\<forall> p. p \<ge> ptr_val (node_next s a) \<longrightarrow>  p \<notin> ptr_span a"
+      by (meson \<open>a < node_next s a\<close> \<open>nodeValid s a\<close> \<open>nodesValid s (node_next s a)\<close> 
+          le_less_trans less_irrefl ptr_less_simp nodeValid_imp_range_l nodesValid.simps(1))
+        
+    hence hrs_the_same_after_a:
+      "\<forall> p. p \<ge> ptr_val (node_next s a) \<longrightarrow> hrs_the_same_at s ?new_s p"
+      using hrs_the_same_except_a by simp
+    with `nodesValid s (node_next s a)` 
+    have "nodesValid ?new_s (node_next s a)"     
+      using nodesValid_heaps_eq_imp_nodesValid by blast
+    hence "nodesValid ?new_s (node_next ?new_s a)" using next_eq by argo
+    hence "nodesValid ?new_s a" using `nodeValid ?new_s a`  nodesValid.simps by blast
+  }
+  ultimately have "nodesValid ?new_s a" by blast
+  moreover have hrs_the_same_before_a: "\<forall> p. p< ptr_val a \<longrightarrow> hrs_the_same_at s ?new_s p" 
+    apply (subgoal_tac "\<forall> p \<in> ptr_span a. p \<ge> ptr_val a")
+    using hrs_the_same_except_a apply force apply auto
+    using `c_guard a` unfolding c_guard_def c_null_guard_def apply auto
+    by (erule zero_not_in_intvl_lower_bound, assumption)
+  hence hrs_the_same_heap_to_a:
+    "\<forall>p. p\<ge> ptr_val ?heap_node \<and> p < ptr_val a \<longrightarrow> hrs_the_same_at s ?new_s p"
+    by blast
+  have "\<forall> p \<in> set (path ?new_s ?heap_node a). nodeValid ?new_s p" 
+    using nodesValid_heaps_eq_nodeValid_in_path
+    using `nodesValid s ?heap_node` hrs_the_same_heap_to_a
+      `reachable s ?heap_node a` `a \<noteq> NULL` 
+    by blast
+  have "reachable ?new_s ?heap_node a" 
+    using hrs_the_same_heap_to_a `reachable s ?heap_node a` `a \<noteq> NULL`      
+    sorry    
+  from reachable have "a \<ge> ?heap_node" 
+    using `a \<noteq> NULL`
+    using reachable_helper2 by presburger
+  moreover {assume "a > ?heap_node"
+    hence "a \<noteq> ?heap_node" by simp
+    hence "node_next s ?heap_node > ?heap_node"
+      using `a > ?heap_node` reachable reachable.elims(2)
+    proof - (* sledgehammered *)
+      { assume "next_C (h_val (hrs_mem (t_hrs_' s)) ?heap_node) \<noteq> a"
+        then have "?heap_node \<noteq> a \<and> ?heap_node \<noteq> a \<and> next_C (h_val (hrs_mem (t_hrs_' s)) ?heap_node) \<noteq> a"
+          using \<open>a \<noteq> ?heap_node\<close> by presburger
+        then have ?thesis
+          using reachable sable_isa.reachable.elims(2) by blast }
+      then show ?thesis
+        using \<open>?heap_node < a\<close> by blast
+    qed 
+    have "node_next s ?heap_node \<le> a"
+      using reachable reachable_next_le_to `a \<noteq> NULL` `a \<noteq> ?heap_node`
       by blast
-  moreover have "\<forall> p \<in> set (path ?new_s (ptr_coerce heap) a). nodeValid ?new_s p" 
-    sorry
-  moreover have "reachable ?new_s (ptr_coerce heap) a" 
-     
-    sorry
-  moreover have "nodeValid ?new_s (ptr_coerce heap)"
-    sorry
-  ultimately have "nodesValid ?new_s (ptr_coerce heap)" using nodesValid_l2 by blast
-  thus "nodesValid ?new_s (ptr_coerce heap)" unfolding heap_invs_def by blast
+    from `nodeValid s ?heap_node` 
+    have "unat_ptr ?heap_node + 8 \<le> unat_ptr (node_next s ?heap_node)"
+      using `node_next s ?heap_node > ?heap_node`
+      apply (simp add: ptr_le_simp ptr_less_simp)
+      apply (drule nodeValid_next_val)
+      by auto
+    hence "unat_ptr ?heap_node + 8 \<le> unat_ptr a"
+      using `node_next s ?heap_node \<le> a`
+      using le_trans ptr_le_simp word_le_nat_alt by blast
+    moreover have "\<forall>p \<in> ptr_span ?heap_node . unat p < unat_ptr ?heap_node + 8"
+      apply (subst eight_eq_eight[THEN sym])
+      apply auto
+      by (erule intvl_upper_bound)
+    ultimately have "\<forall>p \<in> ptr_span a. p \<notin> ptr_span ?heap_node"
+      apply auto
+      apply (subgoal_tac "p \<ge> ptr_val a")
+       apply (meson le_def le_trans word_le_nat_alt)
+      using `c_guard a` unfolding c_guard_def c_null_guard_def
+      apply auto
+      apply (erule zero_not_in_intvl_lower_bound) by assumption
+    hence "\<forall>p \<in> ptr_span ?heap_node. hrs_the_same_at s ?new_s p"
+      using hrs_the_same_except_a by blast
+    hence heap_node_the_same:"node_val s ?heap_node = node_val ?new_s ?heap_node"
+      using hrs_the_same_nodes_the_same by blast
+    hence "node_next ?new_s ?heap_node \<le> a"
+      using `node_next s ?heap_node \<le> a` by simp
+    hence "?heap_node \<in> set (path ?new_s ?heap_node a)" 
+      using path.simps(2)
+      apply (subgoal_tac "?heap_node \<noteq> NULL") 
+       apply (subgoal_tac "?heap_node < node_next ?new_s ?heap_node")
+        apply fastforce
+      using `?heap_node < node_next s ?heap_node` heap_node_the_same apply simp
+      using `c_guard ?heap_node` c_guard_NULL by fast          
+    hence "nodeValid ?new_s ?heap_node"
+      using `\<forall> p \<in> set (path ?new_s ?heap_node a). nodeValid ?new_s p`
+      by fast
+    have "nodesValid ?new_s ?heap_node" using path_nodeValid_reachable_imp_nodesValid
+      using `\<forall> p \<in> set (path ?new_s ?heap_node a). nodeValid ?new_s p`
+        `nodeValid ?new_s ?heap_node`
+        `reachable ?new_s ?heap_node a`
+        `nodesValid ?new_s a` by fast
+  }
+  moreover{
+    assume "?heap_node = a"
+    hence "nodesValid ?new_s ?heap_node"
+      using `nodesValid ?new_s a` by simp
+  }    
+  ultimately show "nodesValid ?new_s ?heap_node" by fastforce
 next 
   fix a::"mem_node_C ptr"
   fix s::globals
-  let ?node_size_masked = "node_size s a && scast (~~ MEM_NODE_OCCUPIED_FLAG)"
-  let ?new_size =  "((size_bytes >> (3::nat)) + (1::32 word) || scast MEM_NODE_OCCUPIED_FLAG)"
-  let ?new_size_masked = "?new_size && scast (~~ MEM_NODE_OCCUPIED_FLAG)"
+  let ?node_size_masked = "node_size s a && scast (~~ OCC_FLG)"
+  let ?new_size =  "((size_bytes >> 3) + 1 || scast OCC_FLG)"
+  let ?new_size_masked = "?new_size && scast (~~ OCC_FLG)"
   let ?new_next = "a +\<^sub>p uint ( 2 + (size_bytes >>3) )"
-  let ?new_next_size ="((size_C (h_val (hrs_mem (t_hrs_' s)) a) && scast (~~ MEM_NODE_OCCUPIED_FLAG)) -
-                 ((2::32 word) + (size_bytes >> (3::nat))) &&
-                 scast (~~ MEM_NODE_OCCUPIED_FLAG))"
-  let ?next = "(next_C (h_val (hrs_mem (t_hrs_' s)) a))"
-  let ?new_s = "(t_hrs_'_update
+  let ?new_next_size = "(?node_size_masked - (2 + (size_bytes >> 3))) && scast (~~ OCC_FLG)"
+  let ?next = "node_next s a"
+  let ?new_s_real = "(t_hrs_'_update
           (hrs_mem_update
             (heap_update a (mem_node_C ?new_size ?new_next)) \<circ>
            hrs_mem_update
             (heap_update ?new_next (mem_node_C ?new_next_size ?next)))
           s)"
-  let ?new_s_simp = 
+  let ?new_s = 
     "(update_node (update_node s ?new_next (mem_node_C ?new_next_size ?next)) a (mem_node_C ?new_size ?new_next))"   
+  let ?heap_node = "(ptr_coerce heap) :: (mem_node_C ptr)"
   assume nodesValid:"nodesValid s (ptr_coerce heap)"
-    "reachable s (ptr_coerce heap) a"
-    "(size_bytes >> 3) + 1  \<le> ?node_size_masked"
-    "node_size s a && scast MEM_NODE_OCCUPIED_FLAG = 0"
-    "(size_bytes >> 3) + 1  < ?node_size_masked"
-    "c_guard a"
-    "a \<noteq> NULL"
-    "c_guard ?new_next"
-  from nodesValid have "a \<ge> (ptr_coerce heap)" using `reachable s (ptr_coerce heap) a` 
-    sorry 
-  have "(1::int) + uint (1 + (size_bytes >>3)) < 2 ^ LENGTH(32)" sorry     
+    and "reachable s (ptr_coerce heap) a"
+    and "(size_bytes >> 3) + 1  \<le> ?node_size_masked"
+    and "node_size s a && scast OCC_FLG = 0"
+    and "(size_bytes >> 3) + 1  < ?node_size_masked"
+    and "c_guard a"
+    and "a \<noteq> NULL"
+    and "c_guard ?new_next"
+  from nodesValid have "a \<ge> (ptr_coerce heap)" 
+    using `reachable s (ptr_coerce heap) a` `a \<noteq> NULL`
+      reachable_helper2 by blast
+  have "1 + uint (1 + (size_bytes >>3)) < 2 ^ LENGTH(32)" sorry     
   hence "uint (2 + (size_bytes >>3) ) =  1 + uint (1 + (size_bytes >>3))" by uint_arith
   hence "ptr_val a + of_int( (uint (2 + (size_bytes >>3) )) * xx) = 
          ptr_val a + of_int( (1 + uint ((size_bytes >>3) + 1)) * xx)" by simp 
@@ -953,13 +1191,400 @@ next
       
   have "?new_next \<noteq> NULL" using `c_guard ?new_next` c_guard_NULL by auto
   have "nodeValid s a" using nodesValid `reachable s (ptr_coerce heap) a` `a \<noteq> NULL`
-    using nodesValid_reachable_imp_nodeValid by blast
-  have size_mem_node_c[simp]:"size_of (TYPE(mem_node_C)) = 8" by simp 
-  have new_s_simp[simp]: "?new_s_simp = ?new_s" by simp
-  have new_size[simp]: "node_size ?new_s a= ?new_size " by (metis new_s_simp updated_node_size)
-  have new_next[simp]: "node_next ?new_s a= ?new_next " by (metis new_s_simp updated_node_next)
-  have "nodeValid ?new_s ?new_next" unfolding nodeValid_def sorry  
-  hence "nodesValid ?new_s ?new_next" sorry
+    using nodesValid_reachable_imp_nodeValid by blast 
+  have new_s_simp[simp]: "?new_s = ?new_s_real" by simp
+  have new_size[simp]: "node_size ?new_s a= ?new_size " by (metis updated_node_size)
+  have new_next[simp]: "node_next ?new_s a= ?new_next " by (metis updated_node_next)
+      
+  have "\<forall>p \<ge> ptr_val ?new_next. hrs_the_same_at s ?new_s p" sorry    
+  have "?next \<noteq> NULL \<longrightarrow> ?next > a" using `nodeValid s a` nodeValid_def by meson
+  have "?next = node_next ?new_s ?new_next"  sorry (* easy *)
+  have "?new_next_size = node_size_masked ?new_s ?new_next " sorry   (* easy *) 
+  have "unat ((size_bytes >> 3) + 1) * 8 < 2 ^ LENGTH(32)"
+    apply (subgoal_tac "unat ?node_size_masked * 8 < 2 ^ LENGTH(32)")
+    using `(size_bytes >> 3) + 1 < ?node_size_masked` 
+     apply unat_arith
+    using `nodeValid s a` unfolding nodeValid_def by meson
+  have "unat ?node_size_masked * 8 < 2 ^ LENGTH(32)"
+    using `nodeValid s a` unfolding nodeValid_def by meson 
+  hence "unat (((size_bytes >> 3) + 1) * 8) = unat ((size_bytes >> 3) + 1) * 8"
+    using \<open>unat ((size_bytes >> 3) + 1) * 8 < 2 ^ LENGTH(32)\<close>
+    by (metis  sable_isa.eight_eq_eight unat_of_nat_eq word_arith_nat_mult)
+  have "unat (?node_size_masked * 8) = unat ?node_size_masked * 8"
+    using `unat ?node_size_masked * 8 < 2 ^ LENGTH(32)`
+    by (metis  sable_isa.eight_eq_eight unat_of_nat_eq word_arith_nat_mult)   
+      
+  {
+    assume "?next \<noteq> NULL"
+    hence "?next > a" using `?next \<noteq> NULL \<longrightarrow> ?next > a` by fast
+        
+    have "unat ?node_size_masked * 8 = unat (?node_size_masked * 8)"
+      using \<open>nodeValid s a\<close> unfolding nodeValid_def Let_def
+      by (metis sable_isa.eight_eq_eight unat_of_nat_eq word_arith_nat_mult)    
+    have 1:"unat_ptr a + 8 + unat ?node_size_masked * 8 \<le> unat_ptr ?next" 
+      using `nodeValid s a` `?next \<noteq> NULL` unfolding nodeValid_def Let_def
+      apply (subst `unat ?node_size_masked * 8 = unat (?node_size_masked * 8)`)
+      by presburger
+        
+    have "unat ((size_bytes >> 3) + 1) * 8 = unat (((size_bytes >> 3) + 1) * 8)"
+      using `unat ((size_bytes >> 3) + 1) * 8 < 2 ^ LENGTH(32)`
+      by (metis sable_isa.eight_eq_eight unat_of_nat_eq word_arith_nat_mult)
+    have "unat_ptr a + 8 + unat (((size_bytes >> 3) + 1) * 8) = unat_ptr ?new_next" 
+      sorry (* proved later *)
+    have 2:"unat_ptr a + 8 + unat ((size_bytes >> 3) + 1) * 8 = unat_ptr ?new_next"
+      apply (insert `unat_ptr a + 8 + unat (((size_bytes >> 3) + 1) * 8) = unat_ptr ?new_next`)
+      by(subst `unat ((size_bytes >> 3) + 1) * 8 = unat (((size_bytes >> 3) + 1) * 8)`)
+        
+    from `(size_bytes >> 3) + 1  < ?node_size_masked`
+    have "unat ((size_bytes >> 3) + 1) * 8 + 8 \<le> unat ?node_size_masked * 8" by unat_arith
+    hence "unat_ptr ?next \<ge> unat_ptr ?new_next + 8" 
+      using 1 2 by unat_arith
+    hence "unat_ptr ?next > unat_ptr ?new_next" by arith
+    hence "?next > ?new_next"
+      apply (simp add:ptr_less_simp) 
+      using unat_less_impl_less by blast
+    have "?next \<ge> ?new_next +\<^sub>p1"
+      using `unat_ptr ?next \<ge> unat_ptr ?new_next + 8` unfolding ptr_add_def 
+      apply (simp only:ptr_val_def ptr_le_simp mem_node_C_size)
+      by (metis mult_numeral_1 numeral_One of_int_numeral of_nat_numeral 
+          eight_eq_eight unat_addition_le_pres)   
+    have "?next > ?new_next \<and> ?next \<ge> ?new_next +\<^sub>p 1 "
+      using `?next \<ge> ?new_next +\<^sub>p1` `?next > ?new_next` by presburger
+  } note next_new_next_rel = this 
+  {
+    have "( 2 + (size_bytes >> 3)) && scast OCC_FLG = 0"
+      apply(subgoal_tac "2 + (size_bytes >> 3) && mask 31 = 2 + (size_bytes >> 3) ")
+       apply(subgoal_tac "scast OCC_FLG && ((mask 31)::32 word) = 0")
+        apply (metis (no_types, hide_lams) word_bw_comms(1) word_bw_lcs(1) word_log_esimps(1))  
+      unfolding MEM_NODE_OCCUPIED_FLAG_def 
+       apply (subgoal_tac "scast (0x80000000 :: 32 signed word) = (1<<31 ::32 word)")
+        apply (metis shiftl_mask_is_0)
+       apply simp
+      apply (subgoal_tac "2 + (size_bytes >> 3)  \<le> mask 31")
+       apply (simp add: and_mask_eq_iff_le_mask)
+      apply (subgoal_tac "(size_bytes >> 3) \<le> 0x1FFFFFFF")     
+      unfolding mask_def apply unat_arith
+      by (rule shiftr3_upper_bound)
+    hence "2 + (size_bytes >> 3) && scast (~~ OCC_FLG) = 2 + (size_bytes >> 3)"
+      by (simp add: sable_isa.l11 sable_isa.mask_sw32_eq_0_eq_x) (* useless? *)
+        
+    have "8 + unat ?node_size_masked * 8 < 2 ^ LENGTH(32)" 
+      using `nodeValid s a` nodeValid_node_size_l3 by blast
+    have node_node_size_bound: "unat (ptr_val a) + 8 + unat (?node_size_masked * 8) 
+      \<le> (if ?next \<noteq> NULL then unat (ptr_val ?next) else 2 ^ LENGTH(32))" 
+      using `nodeValid s a` unfolding nodeValid_def Let_def by simp 
+    have node_node_size_bound_weak:"unat (ptr_val a)+ 8+ unat (?node_size_masked* 8) \<le> 2^ LENGTH(32)" 
+      using \<open>nodeValid s a\<close> sable_isa.nodeValid_node_size_l1_new by blast
+    have "2 + (size_bytes >> 3) \<le> ?node_size_masked"
+      using `(size_bytes >> 3) + 1  < ?node_size_masked` by unat_arith
+    have "?new_next_size = ?node_size_masked - (2 + (size_bytes >> 3))"
+      apply(subgoal_tac "?node_size_masked && (scast OCC_FLG) = 0")
+       apply (subgoal_tac "?node_size_masked - (2 + (size_bytes >> 3)) \<le> ?node_size_masked")
+        apply(subgoal_tac "(?node_size_masked - (2 + (size_bytes >> 3))) && scast OCC_FLG = 0")
+      using sable_isa.mask_sw32_eq_0_eq_x apply blast
+      using OCC_FLAG_helper1 apply blast
+      using `2 + (size_bytes >> 3) \<le> ?node_size_masked` 
+      using word_not_le word_sub_less_iff apply blast
+      using OCC_FLG_neg and_and_not
+      by (metis (no_types, hide_lams) word_bool_alg.conj_left_commute word_bw_comms(1))
+        
+    have "8 + ((size_bytes >> 3) + 1) * 8 < 8 + (?node_size_masked ) * 8"
+      using `(size_bytes >> 3) + 1  < ?node_size_masked`
+      apply (subgoal_tac "8 + unat (?node_size_masked) * 8 < 2 ^ LENGTH(32)")
+       apply(subgoal_tac "unat (8 + ((size_bytes >> 3) + 1) * 8) \<le> 8 + unat ((size_bytes >> 3) + 1) * 8")
+        prefer 3
+      using \<open>8 + unat (?node_size_masked ) * 8 < 2 ^ LENGTH(32)\<close> apply linarith
+       apply (subgoal_tac "unat (8 + ?node_size_masked * 8) = 8 + unat ?node_size_masked * 8")
+        prefer 2
+      using \<open>nodeValid s a\<close>
+        apply (metis (no_types) nodeValid_def eight_eq_eight unat_add_lem unat_mult_lem)
+       apply (subgoal_tac "8 + unat ((size_bytes >> 3) + 1) * 8 < 8 + unat (?node_size_masked) * 8")
+        apply (simp add: word_less_nat_alt)
+       defer
+       apply (subgoal_tac "unat (8 + ((size_bytes >> 3) + 1) * 8) \<le> unat 8 + unat (((size_bytes >> 3) + 1) * 8)")
+        prefer 2
+      using unat_add_le apply blast 
+    proof - (* sledgehammered *)
+      have f1: "\<And>w. unat (8 + (w::32 word)) \<le> 8 + unat w"
+        by (metis sable_isa.eight_eq_eight unat_add_le)
+      then have "\<And>w. unat (8 + (w::32 word)) \<le> 8 + 2 ^ len_of (TYPE(32)::32 itself)"
+        by (meson add_le_cancel_left le_trans nat_less_le unat_lt2p)
+      then have "\<And>n w. n \<le> 8 + 2 ^ len_of (TYPE(32)::32 itself) \<or> \<not> n \<le> unat (8 + (w::32 word))"
+        using le_trans by blast
+      then show "unat (8 + ((size_bytes >> 3) + 1) * 8) \<le> 8 + unat ((size_bytes >> 3) + 1) * 8"
+        using f1 by (metis (no_types) add_le_cancel_left nat_le_linear nat_less_le eight_eq_eight unat_mult_lem)
+    next 
+      have f1: "\<And>w wa. nat (uint (w::32 word)) < nat (uint wa) \<or> \<not> w < wa"
+        by (simp add: unat_def word_less_nat_alt)
+      have "1 + (size_bytes >> 3) < scast (~~ OCC_FLG) && node_size s a"
+        by (metis \<open>(size_bytes >> 3) + 1 < node_size s a && scast (~~ OCC_FLG)\<close> add.commute word_bw_comms(1))
+      then have "8 + 8 * nat (uint (1 + (size_bytes >> 3))) < 8 + 8 * nat (uint (scast (~~ OCC_FLG) && node_size s a))"
+        using f1 by auto
+      then show "8 + unat ((size_bytes >> 3) + 1) * 8 < 8 + unat (size_C (h_val (hrs_mem (t_hrs_' s)) a) && scast (~~ OCC_FLG)) * 8"
+        by (simp add: add.commute unat_def word_bw_comms(1))
+    qed
+      
+    hence "unat (ptr_val a) + unat (8 + ((size_bytes >> 3) + 1) * 8) < 2 ^ LENGTH(32)"
+      using node_node_size_bound_weak by unat_arith
+    hence 1:"unat (ptr_val a + (0x10 + (size_bytes >> 3) * 8)) =
+         unat (ptr_val a) + unat (0x10 + (size_bytes >> 3) * 8)"
+      apply simp
+      using unat_add_lem by fastforce
+        
+    have "?node_size_masked * 8 \<ge>  0x10 + (size_bytes >> 3) * 8"
+      using `(size_bytes >> 3) + 1  < ?node_size_masked`
+      using `2 + (size_bytes >> 3) \<le> ?node_size_masked`
+      apply (subgoal_tac "unat ?node_size_masked * unat (8::32 word) < 2 ^ LENGTH(32)") defer 
+      using `8 + unat ?node_size_masked * 8 < 2 ^ LENGTH(32)` apply unat_arith
+      apply (subgoal_tac "(2 + (size_bytes >> 3)) * 8 \<le> ?node_size_masked * 8") defer
+       apply (rule word_mult_le_mono1)
+      by auto
+        
+    hence 2: "unat(?node_size_masked * 8) \<ge>  unat (0x10 + (size_bytes >> 3) * 8)"
+      using word_le_nat_alt by blast
+        
+    have 3: "unat (?node_size_masked * 8 - (0x10 + (size_bytes >> 3) * 8)) =
+      unat (?node_size_masked * 8) - unat ((0x10 + (size_bytes >> 3) * 8))"
+      using `?node_size_masked * 8 \<ge>  0x10 + (size_bytes >> 3) * 8`
+      using unat_sub by fast
+        
+    have "unat_ptr a + 8 + unat (?node_size_masked * 8) = 
+          unat_ptr ?new_next + 8 + unat ((?node_size_masked - (2 + (size_bytes >> 3))) * 8)"
+      unfolding ptr_add_def
+      apply (simp)
+      by (simp add:1 2 3)
+        
+    hence "unat_ptr ?new_next + 8 + unat (?new_next_size * 8) =
+          unat_ptr a + 8 + unat (?node_size_masked * 8)"
+      apply (subst `?new_next_size = (?node_size_masked - (2 + (size_bytes >> 3)))`)
+      by (rule sym)
+        
+    hence "unat_ptr ?new_next + 8 + unat (?new_next_size * 8) \<le> 
+            (if ?next \<noteq> NULL then unat_ptr ?next else 2 ^ LENGTH(32))" 
+      using node_node_size_bound by simp
+        
+    hence "unat_ptr ?new_next + 8 + unat (?new_next_size * 8) \<le> 
+            (if node_next ?new_s ?new_next \<noteq> NULL then unat_ptr (node_next ?new_s ?new_next) else 2 ^ LENGTH(32))"
+      using `?next = node_next ?new_s ?new_next` by presburger
+        
+    have "nodeFree s a" 
+      using `node_size s a && scast OCC_FLG = 0` `nodeValid s a` sorry (* easy *)
+        
+    have "unat (node_size_masked ?new_s ?new_next) * 8 < 2 ^ LENGTH(32)" sorry 
+        
+    have "nodeFree ?new_s ?new_next"
+      unfolding nodeFree_def Let_def
+      using `\<forall>p \<ge> ptr_val ?new_next. hrs_the_same_at s ?new_s p`        
+    proof-
+      have "unat (ptr_val ( a +\<^sub>p 1)) + unat ?node_size_masked * 8 \<le> 2 ^ LENGTH(32)"
+        using `nodeValid s a` nodeValid_node_size_l2 by fast
+      have "\<forall>p \<in> {ptr_val (a +\<^sub>p 1)..+unat ?node_size_masked * size_of TYPE(mem_node_C)}.
+              snd (hrs_htd (t_hrs_' s) p) = Map.empty" using `nodeFree s a` 
+        by (simp add: sable_isa.nodeFree_def)
+      with `unat (ptr_val ( a +\<^sub>p 1)) + unat ?node_size_masked * 8 \<le> 2 ^ LENGTH(32)`
+      have 1:"\<forall>p. p \<ge> ptr_val (a +\<^sub>p 1) \<and> unat p < unat_ptr (a +\<^sub>p 1) + unat ?node_size_masked * size_of TYPE(mem_node_C) \<longrightarrow>
+                snd (hrs_htd (t_hrs_' s) p) = Map.empty"
+        by (simp add: sable_isa.intvl_no_overflow2) 
+        
+      {assume "unat_ptr ?new_next + 8 \<ge> 2 ^ LENGTH(32)"
+          
+        have "unat_ptr a + 8 + unat (((size_bytes >> 3) + 1) * 8) + 8 \<le> 2 ^ LENGTH(32)"
+          apply (insert `unat_ptr a + 8 + unat (?node_size_masked * 8) \<le> 2 ^ LENGTH(32)`)
+          apply (subst `unat (((size_bytes >> 3) + 1) * 8) = unat ((size_bytes >> 3) + 1) * 8`)
+          apply (subst (asm) `unat (?node_size_masked * 8) = unat ?node_size_masked * 8`)  
+          using `((size_bytes >> 3) + 1) < ?node_size_masked `
+          by unat_arith
+            
+        have "unat_ptr a + 8 + unat (((size_bytes >> 3) + 1) * 8) = unat_ptr ?new_next" 
+          sorry (* proved later *)
+        have "unat_ptr a + 8 + unat (((size_bytes >> 3) + 1) * 8) + 8 \<ge> 2 ^ LENGTH(32)"
+          using `unat_ptr ?new_next + 8 \<ge> 2 ^ LENGTH(32)`
+          apply (subst (asm)`unat_ptr a + 8 + unat (((size_bytes >> 3) + 1) * 8) = unat_ptr ?new_next`[THEN sym])
+          by assumption
+        hence "unat_ptr a + 8 + unat (((size_bytes >> 3) + 1) * 8) + 8 = 2 ^ LENGTH(32)"
+          using `unat_ptr a + 8 + unat (((size_bytes >> 3) + 1) * 8) + 8 \<le> 2 ^ LENGTH(32)`
+          by linarith
+        have "unat ?node_size_masked * 8 \<ge> unat (((size_bytes >> 3) + 1) * 8) + 8"
+          using `?node_size_masked > ((size_bytes >> 3) + 1)`
+          apply (subst `unat (((size_bytes >> 3) + 1) * 8) = unat ((size_bytes >> 3) + 1) * 8`)
+          by unat_arith
+        hence "unat_ptr a + 8 + unat ?node_size_masked * 8 \<ge> 2 ^ LENGTH(32)"
+          using `unat_ptr a + 8 + unat (((size_bytes >> 3) + 1) * 8) + 8 \<ge> 2 ^ LENGTH(32)`
+          by simp
+        hence "unat_ptr a + 8 + unat ?node_size_masked * 8 = 2 ^ LENGTH(32)"
+          using `unat_ptr a + 8 + unat (?node_size_masked * 8) \<le> 2 ^ LENGTH(32)`
+          apply (subst (asm) `unat (?node_size_masked * 8) = unat ?node_size_masked * 8`)
+          by fastforce
+        hence "unat (((size_bytes >> 3) + 1) * 8) + 8 = unat ?node_size_masked * 8"
+          using `unat_ptr a + 8 + unat (((size_bytes >> 3) + 1) * 8) + 8 = 2 ^ LENGTH(32)`
+          by linarith
+        hence "unat ((size_bytes >> 3) + 1) * 8 + 8 = unat ?node_size_masked * 8"
+          using `unat (((size_bytes >> 3) + 1) * 8) = unat ((size_bytes >> 3) + 1) * 8`
+          by linarith
+        hence "(unat ((size_bytes >> 3) + 1) + 1) * 8 = unat ?node_size_masked * 8"
+          by arith
+        hence "((size_bytes >> 3) + 1) + 1 = ?node_size_masked" 
+          by unat_arith
+        hence "?new_next_size = 0"  
+          using `(size_bytes >> 3) + 1  < ?node_size_masked`
+          by simp
+        hence "array_span (?new_next +\<^sub>p 1) (unat ?new_next_size) = {}" by simp     
+        hence "array_span (?new_next +\<^sub>p 1) (unat (node_size_masked ?new_s ?new_next)) = {}"
+          using `?new_next_size = node_size_masked ?new_s ?new_next` by argo
+        hence "\<forall>p \<in> array_span (?new_next +\<^sub>p 1) (unat (node_size_masked ?new_s ?new_next)).
+                 snd (hrs_htd (t_hrs_' ?new_s) p) = Map.empty" by blast
+      }
+      moreover{
+        assume "unat_ptr ?new_next + 8 < 2 ^ LENGTH(32)"
+        hence "unat_ptr (?new_next +\<^sub>p 1) = unat_ptr ?new_next + 8"
+          unfolding ptr_add_def apply (simp only:ptr_val_def mem_node_C_size)
+          using eight_eq_eight
+          by (metis mult_numeral_1 numeral_One of_int_1 unat_of_nat_eq 
+              word_arith_nat_add word_unat.Rep_inverse)
+        have "unat_ptr a + 8 + unat (((size_bytes >> 3) + 1) * 8) = unat_ptr ?new_next" 
+          sorry (* proved later *)
+        hence "?new_next > a"
+          apply (simp add:ptr_less_simp) by unat_arith
+            
+            
+        have "unat (ptr_val (a +\<^sub>p 1)) = unat (ptr_val a + 8)"
+          unfolding ptr_add_def by simp
+            
+        have 2: "ptr_val (?new_next +\<^sub>p 1) > ptr_val ( a +\<^sub>p 1)"  
+          apply (rule TypHeapSimple.unat_less_impl_less)
+          apply (subst `unat_ptr (?new_next +\<^sub>p 1) = unat_ptr ?new_next + 8`)
+          using `?new_next > a`
+          apply (simp only:ptr_less_simp)
+          apply (subst `unat (ptr_val (a +\<^sub>p 1)) = unat (ptr_val a + 8)`) 
+          by unat_arith 
+            
+        have "unat_ptr a + 8 < 2 ^ LENGTH(32)"
+          apply (insert \<open>nodeValid s a\<close>) 
+          apply (drule nodeValid_node_size_l2_new)
+          using `(size_bytes >> 3) + 1  < ?node_size_masked` by unat_arith
+        hence "unat_ptr (a +\<^sub>p 1) = unat_ptr a + 8" 
+          unfolding ptr_add_def by unat_arith
+            
+        have "?new_next_size = (?node_size_masked - (2 + (size_bytes >> 3)))"
+          using \<open>?node_size_masked - (2 + (size_bytes >> 3)) && scast (~~ OCC_FLG) =
+                 ?node_size_masked - (2 + (size_bytes >> 3))\<close> by blast 
+        have "unat ?node_size_masked \<ge> unat (2 + (size_bytes >> 3))" 
+          using \<open>2 + (size_bytes >> 3) \<le> ?node_size_masked\<close> word_le_nat_alt by blast  
+        hence "unat (?node_size_masked - (2 + (size_bytes >> 3))) = 
+               unat ?node_size_masked - unat (2 + (size_bytes >> 3))"
+          using `2 + (size_bytes >> 3) \<le> ?node_size_masked` using unat_sub by blast
+            
+        have "unat (1 + ((size_bytes >>3) + 1)) = unat (1::32 word) + unat ((size_bytes >>3) + 1)"
+          using `(size_bytes >> 3) + 1 < ?node_size_masked`
+          by unat_arith 
+        hence "unat (2 + (size_bytes >>3)) = 1 + unat ((size_bytes >>3) + 1)"
+          by simp
+            
+            
+        have "unat (((size_bytes >> 3) + 1) * 8) = unat ((size_bytes >> 3) + 1) * 8"
+          using `unat ((size_bytes >> 3) + 1) * 8 < 2 ^ LENGTH(32)`
+          by (metis sable_isa.eight_eq_eight unat_mult_lem)
+            
+        have "unat_ptr ?new_next = unat_ptr a + unat (2 + (size_bytes >>3)) * 8"
+          apply (subst `unat (2 + (size_bytes >>3)) = 1 + unat ((size_bytes >>3) + 1)`)
+          apply (subst `unat_ptr a + 8 + unat (((size_bytes >> 3) + 1) * 8) = unat_ptr ?new_next`[THEN sym])
+          apply (subst `unat (((size_bytes >> 3) + 1) * 8) = unat ((size_bytes >> 3) + 1) * 8`) 
+          by auto 
+            
+            (*            hence "node_next ?new_s ?new_next\<ge> ?new_next +\<^sub>p 1" using `?next = node_next ?new_s ?new_next`     
+            sorry 
+               *)
+        have "unat_ptr (?new_next +\<^sub>p 1) + unat ?new_next_size * size_of TYPE(mem_node_C)
+               = unat_ptr (a +\<^sub>p 1) + unat ?node_size_masked * size_of TYPE(mem_node_C)" 
+          apply (subst `unat_ptr (?new_next +\<^sub>p 1) = unat_ptr ?new_next + 8`)
+          apply (subst `unat_ptr ?new_next = unat_ptr a + unat (2 + (size_bytes >>3)) * 8`)
+          apply (subst `unat_ptr (a +\<^sub>p 1) = unat_ptr a + 8`)
+          apply (subst `?new_next_size = (?node_size_masked - (2 + (size_bytes >> 3)))`)
+          apply (subst `unat (?node_size_masked - (2 + (size_bytes >> 3))) = 
+                         unat ?node_size_masked - unat (2 + (size_bytes >> 3))`)
+          using `unat ?node_size_masked \<ge> unat (2 + (size_bytes >> 3))`
+          by auto
+            
+        hence 3: "unat_ptr (?new_next +\<^sub>p 1) + unat (node_size_masked ?new_s ?new_next) * size_of TYPE(mem_node_C)
+                    = unat_ptr (a +\<^sub>p 1) + unat ?node_size_masked * size_of TYPE(mem_node_C)" 
+          using `?new_next_size = node_size_masked ?new_s ?new_next`
+          by argo
+            
+        hence 4: 
+          "unat_ptr (?new_next +\<^sub>p 1)+ (unat (node_size_masked ?new_s ?new_next))* size_of TYPE(mem_node_C) \<le> 
+           2 ^ LENGTH(32)"
+          using \<open>nodeValid s a\<close> nodeValid_node_size_l2 by auto
+        hence "\<forall>p. p \<ge> ptr_val (?new_next +\<^sub>p 1) \<and> 
+                   unat p<unat_ptr (?new_next +\<^sub>p 1) + (unat (node_size_masked ?new_s ?new_next)) * size_of TYPE(mem_node_C) \<longrightarrow> 
+                  p \<ge> ptr_val (a +\<^sub>p 1) \<and> unat p < unat_ptr (a +\<^sub>p 1) + unat ?node_size_masked * size_of TYPE(mem_node_C)"
+          using  2 3 by force
+            
+        hence "\<forall>p \<in> array_span (?new_next +\<^sub>p 1) (unat (node_size_masked ?new_s ?new_next)).
+                 p \<ge> ptr_val (a +\<^sub>p 1) \<and> unat p < unat_ptr (a +\<^sub>p 1) + unat ?node_size_masked * size_of TYPE(mem_node_C)"
+          using 4 apply clarify          
+          apply (drule_tac x=p in intvl_no_overflow2) by blast
+        hence "\<forall>p \<in> array_span (?new_next +\<^sub>p 1) (unat (node_size_masked ?new_s ?new_next)).
+                 snd (hrs_htd (t_hrs_' ?new_s) p) = Map.empty" 
+          using 1 by fastforce
+      }
+      ultimately show "\<forall>p \<in> array_span (?new_next +\<^sub>p 1) (unat (node_size_masked ?new_s ?new_next)).
+                         snd (hrs_htd (t_hrs_' ?new_s) p) = Map.empty" by linarith 
+    qed
+    hence "node_is_occupied ?new_s ?new_next = 0 \<longrightarrow> nodeFree ?new_s ?new_next" by blast
+        
+        
+    have "node_next ?new_s ?new_next \<noteq> NULL \<longrightarrow>(
+          (node_next ?new_s ?new_next) > ?new_next \<and> (node_next ?new_s ?new_next) \<ge> ?new_next +\<^sub>p 1)"
+      using next_new_next_rel
+      using `?next = node_next ?new_s ?new_next` by argo
+        
+    have "nodeValid ?new_s ?new_next" 
+      using `unat_ptr ?new_next + 8 + unat (?new_next_size * 8) \<le> 
+            (if node_next ?new_s ?new_next \<noteq> NULL then unat_ptr (node_next ?new_s ?new_next) else 2 ^ LENGTH(32))`
+        `c_guard ?new_next`
+        `unat (node_size_masked ?new_s ?new_next) * 8 < 2 ^ LENGTH(32)`
+        `node_next ?new_s ?new_next \<noteq> NULL \<longrightarrow>(
+          (node_next ?new_s ?new_next) > ?new_next \<and> (node_next ?new_s ?new_next) \<ge> ?new_next +\<^sub>p 1)`
+        `node_is_occupied ?new_s ?new_next = 0 \<longrightarrow> nodeFree ?new_s ?new_next`
+        `?new_next_size = node_size_masked ?new_s ?new_next`
+      unfolding nodeValid_def
+      by metis
+  }   
+    
+  {
+    assume "?next \<noteq> NULL"
+    hence "?next > a" using `?next \<noteq> NULL \<longrightarrow> ?next > a` by fast
+        
+    hence "\<forall>p \<ge> ptr_val ?next. hrs_the_same_at s ?new_s p"
+      using `?next \<noteq> NULL`[THEN next_new_next_rel, THEN conjunct1]
+      using `\<forall>p \<ge> ptr_val ?new_next. hrs_the_same_at s ?new_s p`
+      by (meson order_less_le_trans ptr_less_def ptr_less_def' word_le_less_eq)
+    have "reachable s ?heap_node ?next"
+      using `reachable s ?heap_node a` `a \<noteq> NULL` nodesValid 
+        nodesValid_reachable_imp_next_reachable by blast 
+    hence "nodesValid s ?next"
+      using `nodesValid s ?heap_node`
+        `?next \<noteq> NULL`
+      using nodesValid_reachable_imp_nodesValid by presburger
+    hence "nodesValid ?new_s ?next"      
+      using nodesValid_heaps_eq_imp_nodesValid
+        `\<forall>p \<ge> ptr_val ?next. hrs_the_same_at s ?new_s p` by blast
+        
+    hence "nodesValid ?new_s ?new_next"
+      using `nodeValid ?new_s ?new_next`
+      using `nodesValid ?new_s ?next`
+      using `?next = node_next ?new_s ?new_next`
+      using nodesValid_def' by metis
+  }
+  moreover{
+    assume "?next = NULL"      
+    hence "nodesValid ?new_s ?new_next"
+      using `nodeValid ?new_s ?new_next`
+        `?next = node_next ?new_s ?new_next`
+        nodesValid_def' by metis
+  }
+  ultimately have "nodesValid ?new_s ?new_next" by satx
+      
   have "unat ?node_size_masked * 8 < 2 ^ LENGTH(32)" 
     using `nodeValid s a` unfolding nodeValid_def by meson
   have node_size_masked_l_2p32:"(unat ?node_size_masked) * unat (8::32 word) < 2 ^ LENGTH(32)" 
@@ -967,66 +1592,68 @@ next
   hence "((size_bytes >> 3) + 1) * 8 < ?node_size_masked * 8"
     using `(size_bytes >> 3) + 1  < ?node_size_masked`
     by (metis eight_eq_eight unat_0 word_gt_0_no word_mult_less_mono1 zero_neq_numeral)          
-  moreover have "unat (ptr_val a) + 8 + unat (?node_size_masked * 8) \<le> 2 ^ LENGTH(32)"
+  moreover have "unat_ptr a + 8 + unat (?node_size_masked * 8) \<le> 2 ^ LENGTH(32)"
     using `nodeValid s a` nodeValid_node_size_l1_new by fast 
-  ultimately have "unat (ptr_val a) + 8 + unat ( ((size_bytes >>3) +1) * 8) <  2 ^ LENGTH(32)"
+  ultimately have "unat_ptr a + 8 + unat ( ((size_bytes >>3) +1) * 8) <  2 ^ LENGTH(32)"
     using `(size_bytes >>3) +1 < ?node_size_masked` `unat ?node_size_masked * 8 < 2 ^ LENGTH(32)`
     by unat_arith
-  moreover have "unat (ptr_val (a+\<^sub>p1)) + unat ( ((size_bytes >>3) +1) * 8) = 
-          unat (ptr_val ((a+\<^sub>p1) +\<^sub>p uint (1 + (size_bytes >> 3))))" 
-    using calculation
-    apply (simp)
-    apply(subgoal_tac "unat (ptr_val (a +\<^sub>p 1)) + unat ((size_bytes >> 3) * 8 + 8) =
-       unat (ptr_val (a +\<^sub>p 1) +( (size_bytes >> 3) * 8 + 8))" )
-     apply(simp)
-    unfolding ptr_add_def
-    by (unat_arith, rule unat_add_lem'[THEN sym], auto)
+
+  have "((size_bytes >> 3) + 1) && scast OCC_FLG = 0"
+    apply(subgoal_tac "(size_bytes >> 3) + 1 && mask 31 = (size_bytes >> 3) + 1")
+    apply(subgoal_tac "scast OCC_FLG && ((mask 31)::32 word) = 0")
+    apply (metis (no_types, hide_lams) word_bw_comms(1) word_bw_lcs(1) word_log_esimps(1))  
+    unfolding MEM_NODE_OCCUPIED_FLAG_def 
+    apply (subgoal_tac "scast (0x80000000 :: 32 signed word) = (1<<31 ::32 word)")
+    apply (metis shiftl_mask_is_0)
+    apply simp
+    apply (subgoal_tac "(size_bytes >> 3) + 1 \<le> mask 31")
+    apply (simp add: and_mask_eq_iff_le_mask)
+    apply (subgoal_tac "(size_bytes >> 3) \<le> 0x1FFFFFFF")     
+    unfolding mask_def apply unat_arith
+    by (rule shiftr3_upper_bound)      
+      
+  hence new_size_eq:"?new_size_masked = (size_bytes >> 3) + 1"
+    by (simp add: sable_isa.l11 sable_isa.mask_sw32_eq_0_eq_x)
+      
+  have "unat_ptr a + 8 + unat (((size_bytes >> 3) + 1) * 8) =
+        unat (ptr_val a + 8 + ((size_bytes >> 3) + 1) * 8)"
+    apply(insert `unat_ptr a + 8 + unat (((size_bytes >> 3) + 1) * 8) < 2 ^ LENGTH(32)`) 
+    using  unat_add_lem_3
+    by (metis sable_isa.eight_eq_eight) 
+  hence "unat_ptr a + 8 + unat (?new_size_masked * 8) = unat_ptr (a +\<^sub>p uint (?new_size_masked + 1))"
+    apply (simp only: new_size_eq)
+    unfolding ptr_add_def apply (simp only: mem_node_C_size)
+    unfolding ptr_val_def apply (simp only: of_int_uint)
+    apply (subst (2) Rings.comm_semiring_class.distrib)
+    by auto 
+  hence "unat_ptr a + 8 + unat (((size_bytes >> 3) + 1) * 8) = unat_ptr ?new_next" 
+    using new_size_eq by auto    
   {      
-      have "unat (ptr_val(a +\<^sub>p 1)) + unat (((size_bytes >>3)+ 1) * 8) < 2 ^ LENGTH(32)"
-        using `(size_bytes >> 3) + 1  < ?node_size_masked` 
-          \<open>unat (ptr_val (a +\<^sub>p 1)) + unat (?node_size_masked * 8) \<le> 2 ^ LENGTH(32)\<close>
-        by (metis \<open>unat (ptr_val (a +\<^sub>p 1)) + unat (((size_bytes >> 3) + 1) * 8) = unat (ptr_val (a +\<^sub>p 1 +\<^sub>p uint (1 + (size_bytes >> 3))))\<close> unat_lt2p)
-      hence "ptr_val(a +\<^sub>p 1) + ((size_bytes >>3)+ 1) * 8  \<ge> ptr_val(a +\<^sub>p 1)"
-        using no_olen_add_nat by blast
-          
-      moreover have "(a +\<^sub>p 1) +\<^sub>p uint ((size_bytes >>3)+ 1) = (a +\<^sub>p 1) +\<^sub>p unat ((size_bytes >>3)+ 1)"
-        by (simp add: uint_nat)
-          
-      ultimately have "ptr_val ?new_next \<ge>  ptr_val (a +\<^sub>p 1)"
-        using `?new_next = (a +\<^sub>p 1) +\<^sub>p uint ((size_bytes >>3)+ 1)` unfolding ptr_add_def
-        by (metis (mono_tags, hide_lams) mem_node_C_size of_int_uint of_nat_numeral ptr_val.ptr_val_def) 
-      hence "?new_next \<ge> (a +\<^sub>p 1)" by (simp add: ptr_le_def ptr_le_def') 
-      moreover have "(a +\<^sub>p 1) > a" sorry (* false! *)
-      ultimately have new_next_g_a:"?new_next > a \<and> ?new_next \<ge> (a +\<^sub>p 1)" using order_less_le_trans by auto 
-    } note  new_next_g_a= this
+    from `unat_ptr a + 8 + unat (((size_bytes >> 3) + 1) * 8) = unat_ptr ?new_next`
+    have "unat_ptr ?new_next \<ge> unat_ptr a + 8"
+      unfolding ptr_add_def
+      by (simp add:ptr_less_simp) 
+    hence "?new_next \<ge> a +\<^sub>p 1" 
+      unfolding ptr_add_def
+      apply (simp add:ptr_le_simp) 
+      apply (subst (asm) eight_eq_eight[THEN sym])
+      by(erule unat_addition_le_pres)  
+    moreover have "?new_next > a" 
+      using `unat_ptr a + 8 + unat (((size_bytes >> 3) + 1) * 8) = unat_ptr ?new_next`
+      apply(simp only:ptr_less_simp)
+      by (simp add: word_less_nat_alt)
+    ultimately have new_next_g_a:"?new_next > a \<and> ?new_next \<ge> (a +\<^sub>p 1)" 
+      using order_less_le_trans by auto 
+  } note new_next_g_a= this
   moreover{
-    have "((size_bytes >> 3) + 1) && scast MEM_NODE_OCCUPIED_FLAG = 0"
-      unfolding MEM_NODE_OCCUPIED_FLAG_def sorry (* obvious *)
-    hence new_size_eq:"?new_size_masked = (size_bytes >> 3) + 1"
-      by (simp add: sable_isa.l11 sable_isa.mask_sw32_eq_0_eq_x)
-    have 1:"unat (ptr_val a) + 8 + unat (?node_size_masked * 8) 
-      \<le> (if ?next \<noteq> NULL then unat (ptr_val ?next) else (2::nat) ^ LENGTH(32))" 
-      using `nodeValid s a` unfolding nodeValid_def Let_def by simp
-    hence "unat (ptr_val a) + 8 + unat (?node_size_masked * 8) 
-      \<le>  unat (ptr_val ?next)" sorry (* easy *)
-    moreover have "unat (ptr_val ((a+\<^sub>p1) +\<^sub>p uint (1 + (size_bytes >> 3)))) =
-           unat (ptr_val (a +\<^sub>p uint (2 + (size_bytes >> 3))))"
-      by (simp add: \<open>a +\<^sub>p uint (2 + (size_bytes >> 3)) = a +\<^sub>p 1 +\<^sub>p uint ((size_bytes >> 3) + 1)\<close> add.commute) 
-      (* \<up> duplicate fact? \<up> *)
-    
-    ultimately have "unat (ptr_val a) + 8 + unat (((size_bytes >> 3) + 1) * 8)
-                     \<le> unat (ptr_val ?new_next)"
-      using  (* `?new_next = (a +\<^sub>p 1) +\<^sub>p uint ((size_bytes >>3)+ 1)` *)
-        `(size_bytes >> 3) + 1  < ?node_size_masked`
-      `unat (ptr_val a) + 8 + unat (((size_bytes >> 3) + 1) * 8) < 2 ^ LENGTH(32)`
-      (* \<open>unat (ptr_val (a +\<^sub>p 1)) + unat (((size_bytes >> 3) + 1) * 8) = 
-       unat (ptr_val (a +\<^sub>p 1 +\<^sub>p uint (1 + (size_bytes >> 3))))\<close>  *)             
-      sorry
-    hence  "unat (ptr_val a) + 8 + unat (?new_size_masked * 8) \<le> unat (ptr_val ?new_next)"
+    from `unat_ptr a + 8 + unat (((size_bytes >> 3) + 1) * 8) = unat_ptr ?new_next`
+    have "unat_ptr a + 8 + unat (((size_bytes >> 3) + 1) * 8) \<le> unat_ptr ?new_next" 
+      by auto         
+    hence  "unat_ptr a + 8 + unat (?new_size_masked * 8) \<le> unat_ptr ?new_next"
       using new_size_eq by argo
-    hence "unat (ptr_val a) + 8 + unat (?new_size_masked * 8)
-       \<le> (if ?new_next \<noteq> NULL then unat (ptr_val ?new_next) else 2 ^ LENGTH(32))"
-    sorry (* easy *)   
+    hence "unat_ptr a + 8 + unat (?new_size_masked * 8)
+       \<le> (if ?new_next \<noteq> NULL then unat_ptr ?new_next else 2 ^ LENGTH(32))"
+      using `?new_next \<noteq> NULL` by simp
     moreover{ have "(unat ?node_size_masked) * 8 < 2 ^ LENGTH(32)" 
         using `nodeValid s a` unfolding nodeValid_def by meson  
       with `(size_bytes >> 3) + 1  < ?node_size_masked` 
@@ -1034,120 +1661,70 @@ next
         apply (subst new_size_eq) apply(drule unat_mono)  by linarith
     }
     moreover{
-      have "node_is_occupied ?new_s a = scast MEM_NODE_OCCUPIED_FLAG"
-        by (metis (no_types) new_s_simp sable_isa.updated_node_size word_ao_absorbs(5))
+      have "node_is_occupied ?new_s a = scast OCC_FLG"
+        by (metis (no_types) sable_isa.updated_node_size word_ao_absorbs(5))
       hence "node_is_occupied ?new_s a \<noteq> 0" unfolding MEM_NODE_OCCUPIED_FLAG_def by auto 
     }
-    moreover  have "(?new_next \<noteq> NULL \<longrightarrow> ?new_next > a \<and> ?new_next \<ge> a +\<^sub>p 1)" using new_next_g_a by auto
+    moreover  have "(?new_next \<noteq> NULL \<longrightarrow> ?new_next > a \<and> ?new_next \<ge> a +\<^sub>p 1)" 
+      using new_next_g_a by auto
     ultimately have "nodeValid ?new_s a" using `c_guard a` unfolding nodeValid_def
       using new_next new_size by auto        
   }      
-  ultimately have "nodesValid ?new_s a" using  new_next  `nodesValid ?new_s ?new_next` 
+  ultimately have "nodesValid ?new_s a" (* !! *)
+    using new_next `nodesValid ?new_s ?new_next` 
     using nodesValid_trans_back by presburger
-      (* have "unat (ptr_val (a +\<^sub>p 1)) + unat (?node_size_masked * 8) \<le> unat (ptr_val ?next)" 
-    using `nodeValid s a` unfolding nodeValid_def  
-    by (simp add: `?next \<noteq> NULL`) *)
-  have "\<forall> p. p < ptr_val a \<longrightarrow> hrs_the_same_at s ?new_s_simp p"
+  have "\<forall> p. p < ptr_val a \<longrightarrow> hrs_the_same_at s ?new_s p"
     apply clarify
     apply (rule updated_node_blahblah_2) using new_next_g_a 
     apply (subgoal_tac "ptr_val a < ptr_val ( a +\<^sub>p uint (2 + (size_bytes >> 3)))")
     by (auto simp:ptr_less_def' ptr_less_def)
-  hence range_imp_hrs_the_same:
-    "\<forall> p. p \<ge> ptr_val (ptr_coerce heap) \<and> p < ptr_val a \<longrightarrow> hrs_the_same_at s ?new_s_simp p"
-    by simp
-      
+  hence hrs_the_same_heap_to_a:
+    "\<forall> p. p \<ge> ptr_val (ptr_coerce heap) \<and> p < ptr_val a \<longrightarrow> hrs_the_same_at s ?new_s p"
+    by simp   
   hence paths_the_same:"path s (ptr_coerce heap) a = path ?new_s (ptr_coerce heap) a"
-    apply (subst new_s_simp[THEN sym]) 
     by (rule heaps_eq_imp_paths_eq)
       
-  have new_s_path_nodeValid:"\<forall> p \<in> set (path ?new_s (ptr_coerce heap) a). nodeValid ?new_s p"
-  proof clarify
-    fix np::"mem_node_C ptr"
-    assume np_in_path:"np \<in> set (path ?new_s (ptr_coerce heap) a)"
-    have "ptr_val np < ptr_val a" 
-      using np_in_path p_in_path_l_to ptr_less_def ptr_less_def' by blast
-    moreover have "ptr_val np \<ge> ptr_val (ptr_coerce heap)" 
-      using np_in_path p_in_path_ge_node ptr_le_def ptr_le_def'
-      by (metis Ptr_ptr_coerce ptr_val.ptr_val_def)        
-    ultimately have "hrs_the_same_at s ?new_s (ptr_val np)" using range_imp_hrs_the_same
-      by simp    
-        
-    have np_in_s_path:"np \<in> set (path s (ptr_coerce heap) a)" using np_in_path paths_the_same by argo    
-    hence "nodeValid s np" using `nodesValid s (ptr_coerce heap)` 
-      node_in_path_nodesValid_imp_nodeValid_node by fast
-    
-    have "node_next s np \<le> a" using np_in_s_path  p_in_path_next_le_to by blast
-    with `nodeValid s np` have "unat (ptr_val (np +\<^sub>p 1)) + unat((node_size_masked s np) * 8) \<le> 
-    ( if (node_next s np \<noteq> NULL) then unat (ptr_val (node_next s np)) else 2 ^ LENGTH(32))"
-      unfolding nodeValid_def sorry (*  by metis *)
-    moreover have "node_next s np \<noteq> NULL" using `nodeValid s np`
-        sorry
-        (* by (metis (no_types) Ptr_not_null_pointer_not_zero Ptr_ptr_coerce  c_guard_NULL nodeValid_def ptr_coerce_NULL reachable.simps reachable_trans word_not_simps(1)) *)
-      (* \<up> suspicious \<up> *)
-    ultimately have "unat (ptr_val (np +\<^sub>p 1)) + unat((node_size_masked s np) * 8) \<le> 
-      unat (ptr_val (node_next s np))" by auto
-    hence "unat (ptr_val (np +\<^sub>p 1)) + unat((node_size_masked s np) * 8) \<le> unat (ptr_val a)"
-      using `node_next s np \<le> a`
-      apply (simp  add: ptr_le_def ptr_le_def')
-      by unat_arith
-    moreover have "unat (node_size_masked s np) * 8 < 2 ^ LENGTH(32)" using `nodeValid s np` 
-      unfolding nodeValid_def by metis
-    ultimately have "\<forall> p \<in> array_span (np +\<^sub>p 1) (unat (node_size_masked s np)). 
-     p < ptr_val a"     
-      unfolding intvl_def
-      apply unat_arith  apply auto
-      apply (subgoal_tac "unat (node_size_masked s np) * 8 < 2 ^ LENGTH(32)")
-       apply (subgoal_tac "unat (of_nat k) = k") 
-        apply(subgoal_tac "unat (node_size_masked s np) * 8 = unat ((node_size_masked s np) * 8)")
-         apply (erule_tac t="unat (of_nat k)" in ssubst) 
-         apply simp
-        apply (metis sable_isa.eight_eq_eight unat_of_nat_eq word_arith_nat_mult)
-       apply (simp add: unat_of_nat_eq)
-      by simp
-    hence "\<forall>p \<in> array_span (np +\<^sub>p 1) (unat (node_size_masked s np)).
-           hrs_the_same_at s ?new_s p" 
-      by (simp add:`\<forall> p <ptr_val a. hrs_the_same_at s ?new_s_simp p`)  
-    from `nodeValid s np` have "\<forall> p \<in> {ptr_val np ..+ size_of (TYPE(mem_node_C))}. p < ptr_val a"
-      using `ptr_val np < ptr_val a`
-        `nodeValid s a` nodeValid_imp_range_l by blast
-    hence "\<forall>p \<in> {ptr_val np ..+ size_of (TYPE(mem_node_C))}. hrs_the_same_at s ?new_s p"
-      by (simp add:`\<forall> p <ptr_val a. hrs_the_same_at s ?new_s_simp p`)
-    moreover have "\<forall>p\<in>{ptr_val (np +\<^sub>p 1) ..+ unat (node_size_masked s np) * size_of TYPE(mem_node_C)}.
-       hrs_the_same_at s ?new_s p" sorry (* not a matter of convincing Isabelle  *)
-    ultimately show "nodeValid ?new_s np" using `nodeValid s np` hrs_the_same_imp_nodeValid by blast  
-  qed     
+  moreover have new_s_path_nodeValid:"\<forall> p \<in> set (path ?new_s ?heap_node a). nodeValid ?new_s p" 
+    using nodesValid_heaps_eq_nodeValid_in_path
+    using `nodesValid s ?heap_node` hrs_the_same_heap_to_a
+      `reachable s ?heap_node a` `a \<noteq> NULL` 
+    by blast    
       
-  moreover have "reachable ?new_s (ptr_coerce heap) a"
-    apply (subst new_s_simp[THEN sym])
+  moreover have "reachable ?new_s ?heap_node a"
     using `reachable s (ptr_coerce heap) a`
       `nodesValid s (ptr_coerce heap)`
-      range_imp_hrs_the_same
-      hrs_the_sam_nodesValid_reachable_imp_reachable by blast
+      hrs_the_same_heap_to_a
+      `a \<noteq> NULL`
+      hrs_the_sam_nodesValid_reachable_imp_reachable by blast     
       
-  moreover{    
-    {assume "a > ptr_coerce heap" 
-      hence "a \<noteq> ptr_coerce heap" by simp
-      hence "(ptr_coerce heap) \<in> set (path s (ptr_coerce heap) a)" 
-        using `nodesValid s (ptr_coerce heap)` `reachable s (ptr_coerce heap) a` `a \<noteq> NULL` 
+  {assume "a > ptr_coerce heap" 
+    hence "a \<noteq> ptr_coerce heap" by simp
+    hence "(ptr_coerce heap) \<in> set (path s (ptr_coerce heap) a)" 
+      using `nodesValid s (ptr_coerce heap)` `reachable s (ptr_coerce heap) a` `a \<noteq> NULL` 
         nodesValid_reachable_imp_in_path by fast
-      hence "(ptr_coerce heap) \<in> set (path ?new_s (ptr_coerce heap) a)"
-        using paths_the_same by argo
-      hence  "nodeValid ?new_s (ptr_coerce heap)" using new_s_path_nodeValid by fast
-    }
-    moreover
-    {assume "\<not>a > ptr_coerce heap"
-      hence "a = ptr_coerce heap" using ` a \<ge>  ( ptr_coerce heap)` by simp
-      hence "nodeValid ?new_s (ptr_coerce heap)" using `nodeValid ?new_s a` by simp
-    }
-    ultimately have "nodeValid ?new_s (ptr_coerce heap)" by blast
+    hence "(ptr_coerce heap) \<in> set (path ?new_s (ptr_coerce heap) a)"
+      using paths_the_same by argo
+    hence  "nodeValid ?new_s (ptr_coerce heap)" using new_s_path_nodeValid by fast
+  } moreover
+  {assume "\<not>a > ptr_coerce heap"
+    hence "a = ptr_coerce heap" using ` a \<ge>  ( ptr_coerce heap)` by simp
+    hence "nodeValid ?new_s (ptr_coerce heap)" using `nodeValid ?new_s a` by simp
   }
-  ultimately have "nodesValid ?new_s (ptr_coerce heap)" using
-      `nodesValid ?new_s a` apply (simp only:`?new_s_simp = ?new_s`[THEN sym]) 
-    (* FIXME: error *)
-    apply (rule nodesValid_l2) by blast+
-  thus "nodesValid ?new_s (ptr_coerce heap)" by auto
+  ultimately have "nodeValid ?new_s (ptr_coerce heap)" by blast
+      
+  have "nodesValid ?new_s ?heap_node" 
+    using `nodesValid ?new_s a`
+      `nodeValid ?new_s ?heap_node`
+      `reachable ?new_s ?heap_node a`
+      new_s_path_nodeValid 
+    apply auto
+    apply (rule path_nodeValid_reachable_imp_nodesValid)
+    by blast+
+  thus "nodesValid ?new_s_real (ptr_coerce heap)" by auto
 qed
- 
+
+
+  
 lemma alloc'_hoare_helper:
   fixes size_bytes heap
   assumes n:"size_of TYPE('a) \<le> unat size_bytes"
@@ -1156,25 +1733,25 @@ lemma alloc'_hoare_helper:
        heap_invs s heap \<Longrightarrow>
        reachable s (ptr_coerce heap) node \<Longrightarrow>
        (size_bytes >> (3::nat)) + (1::32 word)
-       \<le> size_C (h_val (hrs_mem (t_hrs_' s)) node) && scast (~~ MEM_NODE_OCCUPIED_FLAG) \<Longrightarrow>
-       size_C (h_val (hrs_mem (t_hrs_' s)) node) && scast MEM_NODE_OCCUPIED_FLAG = (0::32 word) \<Longrightarrow>
+       \<le> size_C (h_val (hrs_mem (t_hrs_' s)) node) && scast (~~ OCC_FLG) \<Longrightarrow>
+       size_C (h_val (hrs_mem (t_hrs_' s)) node) && scast OCC_FLG = (0::32 word) \<Longrightarrow>
        node \<noteq> NULL \<Longrightarrow>
        c_guard node \<Longrightarrow>      
        ptr_val (node +\<^sub>p (1::int)) \<noteq> (0::32 word) \<Longrightarrow>
        heap_ptr_valid (ptr_retyp ((ptr_coerce (node +\<^sub>p (1)))::'a::mem_type ptr) (hrs_htd (t_hrs_' s)))
         ((ptr_coerce (node +\<^sub>p (1::int))):: 'a ptr)"
-unfolding heap_invs_def
+  unfolding heap_invs_def
 proof -
   fix s :: globals fix node ::"mem_node_C ptr"
   let ?ptrc = "ptr_coerce (node  +\<^sub>p 1) :: 'a ptr"
-  let ?node_size = "size_C (h_val (hrs_mem (t_hrs_' s)) node) && scast (~~ MEM_NODE_OCCUPIED_FLAG) :: 32 word"
+  let ?node_size = "size_C (h_val (hrs_mem (t_hrs_' s)) node) && scast (~~ OCC_FLG) :: 32 word"
   let ?blocks = "(size_bytes >> 3) + 1 :: 32 word"
   let ?heap_ptr = "ptr_coerce heap :: mem_node_C ptr"
   assume "ptr_val (node +\<^sub>p 1) \<noteq> 0" 
     and invs: "nodesValid s (ptr_coerce heap)"
     and blocks_size: "?blocks \<le> ?node_size"
     and "reachable s (ptr_coerce heap) node"
-    and node_empty: "size_C (h_val (hrs_mem (t_hrs_' s)) node) && scast MEM_NODE_OCCUPIED_FLAG = 0"
+    and node_empty: "size_C (h_val (hrs_mem (t_hrs_' s)) node) && scast OCC_FLG = 0"
     and "node \<noteq> NULL"
     and "c_guard node"
     and "ptr_val (node +\<^sub>p 1) \<noteq> 0"
@@ -1184,7 +1761,7 @@ proof -
   hence empty: "\<forall>p\<in>{ptr_val (node +\<^sub>p 1)..+unat ?node_size * 8}.
                             snd (hrs_htd (t_hrs_' s) p) = Map.empty"
     unfolding nodeFree_def by auto
-  have node_size: "unat (ptr_val (node +\<^sub>p 1)) + unat (?node_size * 8) \<le> 2 ^ len_of (TYPE(32))"
+  have node_size: "unat_ptr (node +\<^sub>p 1) + unat (?node_size * 8) \<le> 2 ^ len_of (TYPE(32))"
     using `nodeValid s node`  sable_isa.nodeValid_node_size_l1 by presburger   
   have "0 \<notin> {ptr_val (node +\<^sub>p 1)..+ unat (?node_size * 8)}"
   proof (rule ccontr)
@@ -1193,9 +1770,9 @@ proof -
     then obtain k where 0:"0=ptr_val (node +\<^sub>p 1) + of_nat k \<and> k < unat (?node_size * 8)"
       using intvlD by blast
     hence "k \<le> unat (?node_size * 8) -1 " by (simp add: nat_le_Suc_less_imp)
-    moreover from node_size have "unat (ptr_val (node +\<^sub>p 1)) + (unat (?node_size * 8) - 1) < 2 ^ len_of (TYPE(32))"
+    moreover from node_size have "unat_ptr (node +\<^sub>p 1) + (unat (?node_size * 8) - 1) < 2 ^ len_of (TYPE(32))"
       by unat_arith
-    ultimately have "unat (ptr_val (node +\<^sub>p 1)) +  k <  2 ^ len_of (TYPE(32))" by arith
+    ultimately have "unat_ptr (node +\<^sub>p 1) +  k <  2 ^ len_of (TYPE(32))" by arith
     hence "ptr_val (node +\<^sub>p 1) + of_nat k \<ge> ptr_val (node +\<^sub>p 1)"
       by (metis add.commute add_lessD1 no_olen_add_nat unat_of_nat32 word_bits_def)
     hence "ptr_val (node +\<^sub>p 1) + of_nat k \<noteq> 0" using `ptr_val (node +\<^sub>p 1) \<noteq> 0` by auto
@@ -1211,8 +1788,8 @@ proof -
     show "valid_simple_footprint (ptr_retyp ?ptrc (hrs_htd (t_hrs_' s))) (ptr_val ?ptrc)
           (typ_uinfo_t TYPE('a))"
       apply (rule TypHeapSimple.valid_simple_footprint_ptr_retyp) defer
-        apply (simp, metis Suc_le_eq mem_type_simps(3) size_of_def)
-       apply (simp add: size_of_tag)
+      apply (simp, metis Suc_le_eq mem_type_simps(3) size_of_def)
+      apply (simp add: size_of_tag)
     proof safe 
       fix k
       assume "k < size_td (typ_uinfo_t TYPE('a))"
@@ -1274,78 +1851,78 @@ lemma alloc'_hoare:
   apply (subst whileLoop_add_inv 
       [where I="\<lambda> (n,r) s. heap_invs s heap  \<and> reachable s (ptr_coerce heap) n
                   \<and> (r=0 \<longrightarrow> n = NULL \<or> ((size_bytes >> 3) + 1
-                     \<le> size_C (h_val (hrs_mem (t_hrs_' s)) n) && scast (~~ MEM_NODE_OCCUPIED_FLAG))
-                  \<and> size_C (h_val (hrs_mem (t_hrs_' s)) n) && scast MEM_NODE_OCCUPIED_FLAG = 0)" 
+                     \<le> size_C (h_val (hrs_mem (t_hrs_' s)) n) && scast (~~ OCC_FLG))
+                  \<and> size_C (h_val (hrs_mem (t_hrs_' s)) n) && scast OCC_FLG = 0)" 
         and M="\<lambda> ((n,y),s). ptr_val n"])
   apply (wp fail'_wp)
-      apply (simp add: `0 < size_bytes` h_val_id not_le)
-      defer defer
-      apply (wp fail'_wp)
-     prefer 2
-     apply (erule iffD1[OF refl])
-    apply (auto simp: `0 < size_bytes`)
-                    apply wp
-                    apply auto
-                      (* FIXME error *)
-                      apply (rule self_reachable, solves simp)
-                      apply (drule heap_invs_not_null, solves auto)
-                      apply (rule self_reachable, solves auto)
-                      apply (drule one_mask_neg_MNOF_not_zero, solves simp)
-                      apply (drule heap_invs_not_null, solves auto)
-                      apply (rule self_reachable, solves auto)
-                     apply (drule mask_sw32_eq_0_eq_x, solves auto)
-                    apply (drule heap_invs_not_null, solves auto)
-                    unfolding heap_invs_def
-                    (* FIXME: use this: *)
-                  apply(drule nodesValid_reachable_imp_next_reachable, auto)+
-                   (*instead of this: apply (drule reachable_trans,solves auto, solves auto)+ *)
-                                   apply (drule one_mask_neg_MNOF_not_zero, solves simp)
-                   
-               apply (drule reachable_trans,solves auto, solves auto)
-              apply (drule c_guard_NULL,rule reachable_trans, solves simp, solves simp)
-             apply (drule mask_sw32_eq_0_eq_x, solves auto)
-            apply (drule c_guard_NULL,drule reachable_trans, solves simp, solves simp)+
-        apply (drule one_mask_neg_MNOF_not_zero, solves simp)
-       apply (drule c_guard_NULL,drule reachable_trans, solves simp, solves simp)+
-     apply (drule mask_sw32_eq_0_eq_x, solves auto)
-    apply (drule c_guard_NULL,drule reachable_trans, solves simp, solves simp)
+  apply (simp add: `0 < size_bytes` h_val_id not_le)
+  defer defer
+  apply (wp fail'_wp)
+  prefer 2
+  apply (erule iffD1[OF refl])
+  apply (auto simp: `0 < size_bytes`)
+  apply wp
+  apply auto
+    (* FIXME error *)
+  apply (rule self_reachable, solves simp)
+  apply (drule heap_invs_not_null, solves auto)
+  apply (rule self_reachable, solves auto)
+  apply (drule one_mask_neg_MNOF_not_zero, solves simp)
+  apply (drule heap_invs_not_null, solves auto)
+  apply (rule self_reachable, solves auto)
+  apply (drule mask_sw32_eq_0_eq_x, solves auto)
+  apply (drule heap_invs_not_null, solves auto)
+  unfolding heap_invs_def
+    (* FIXME: use this: *)
+  apply(drule nodesValid_reachable_imp_next_reachable, auto)+
+    (*instead of this: apply (drule reachable_trans,solves auto, solves auto)+ *)
+  apply (drule one_mask_neg_MNOF_not_zero, solves simp)
+    
+  apply (drule reachable_trans,solves auto, solves auto)
+  apply (drule c_guard_NULL,rule reachable_trans, solves simp, solves simp)
+  apply (drule mask_sw32_eq_0_eq_x, solves auto)
+  apply (drule c_guard_NULL,drule reachable_trans, solves simp, solves simp)+
+  apply (drule one_mask_neg_MNOF_not_zero, solves simp)
+  apply (drule c_guard_NULL,drule reachable_trans, solves simp, solves simp)+
+  apply (drule mask_sw32_eq_0_eq_x, solves auto)
+  apply (drule c_guard_NULL,drule reachable_trans, solves simp, solves simp)
   using n align apply (rule alloc'_hoare_helper, auto)
   using n align apply (rule alloc'_hoare_helper, auto) 
   done
- 
-
+    
+    
 text \<open> hello! @{thm (lhs) simple_lift_def}  \<close>   
-
+  
 thm "valid_simple_footprint_def"
 thm "heap_ptr_valid_def"
 thm "simple_lift_def"
 typ "globals"
 print_record "lifted_globals"
 value " (s :: globals)"
-(*declare [[show_types]]
+  (*declare [[show_types]]
 declare [[show_consts]]
 declare [[show_sorts]]*)
-
+  
 lemma alloc_w32_safe: "\<lbrace>\<lambda>s. (liftC lift_global_heap (\<lambda>s. heap_invs s heap)) s\<rbrace>
                        exec_concrete lift_global_heap (alloc' heap 4)
       \<lbrace>\<lambda>r s. ptr_val r \<noteq> 0 \<longrightarrow> is_valid_w32 s ((ptr_coerce r) :: (32 word) ptr)\<rbrace>!"
-apply (rule validNF)
-apply wp
-apply (rule hoare_post_imp)
-prefer 2
+  apply (rule validNF)
+  apply wp
+  apply (rule hoare_post_imp)
+  prefer 2
   apply (rule alloc'_hoare[where 'a="32 word"])
   apply (auto simp add: align_of_def Let_def)+
   apply (simp add: lifted_globals_ext_simps(6) simple_lift_def)
-using alloc'_hoare[where n=4 and 'a="32 word"] apply (simp add: Let_def
-unfolding validNF_def valid_def
-apply auto
+  using alloc'_hoare[where n=4 and 'a="32 word"] apply (simp add: Let_def
+  unfolding validNF_def valid_def
+  apply auto
 proof -
   fix s a b
   assume "\<forall>g. lift_global_heap s = lift_global_heap g \<longrightarrow> heap_invs g"
-     and "\<forall>g. lift_global_heap b = lift_global_heap g \<longrightarrow> heap_invs g"
+    and "\<forall>g. lift_global_heap b = lift_global_heap g \<longrightarrow> heap_invs g"
   hence "heap_invs s" and "heap_invs b" by auto
-oops
-
+  oops
+    
 end
-
+  
 end
